finished proofs and certified books

acl2/books/arithmetic/sum.lisp
@@ -1,27 +1,26 @@
 (in-package "ACL2")
 (include-book "../../erl-eval")
-(include-book "../../theorems/core/top")
-(include-book "../../theorems/state/state")
-(include-book "std/lists/len" :dir :system)
-; some things from state
-; atomic, exprs, binop, functions, local-call
+(include-book "../../theorems/top")
+(include-book "std/omaps/top" :dir :system)
 
 (set-induction-depth-limit 1)
 
-; ACL2 sum-n
-(define sum-n ((n natp))
+; ACL2 sum
+(define sum ((n natp))
   (b* ((n (nfix n))
        ((if (= n 0)) 0))
-      (+ n (sum-n (1- n)))))
+      (+ n (sum (1- n)))))
 
-; Commenting this out, as it introduces rewrite rules that we do 
-; not want yet.
-; (defrule sum-n-formula
-;   (implies (natp n)
-;     (equal (sum-n n) (/ (* n (+ n 1)) 2)))
-;   :enable (sum-n))
-
-(define test-w ()
+;; Erlang World with the following functions defined locally.
+;; - When you run Erlang on the command line, the module is set to 'local.
+;;   Normally, functions like add and would be defined in a different module
+;;   which we would then have to import (or do a remote call m:f()) but I will
+;;   ignore that here for simplicity.
+;;
+;; sum(0) -> 0;
+;; sum(X) when is_integer(X), X > 0 -> X + sum(X - 1).
+;;
+(define sum-test-w ()
   :returns (w world-p)
   :enabled t
   '((local
@@ -44,532 +43,320 @@
                     (:cons (:binop - (:var X) (:integer 1)) 
                            (:nil)))))))))))
 
-(defrule update-erl-state-in-bind-chain-rule
-  (equal (update-erl-state->bind 
-           (update-erl-state->in 
-             (update-erl-state->bind 
-               (update-erl-state->in s v1) 
-                b1)
-              v2)
-            b2)
-         (update-erl-state->bind (update-erl-state->in s v2) b2))
-  :enable (update-erl-state->in update-erl-state->bind))
 
-(defrule update-erl-state-in-bind-chain-rule-2
-  (equal (update-erl-state->bind 
-           (update-erl-state->in (update-erl-state->bind s b1) v)
-            b2)
-         (update-erl-state->bind (update-erl-state->in s v) b2))
-  :enable (update-erl-state->in update-erl-state->bind))
-
-(defrule update-erl-state-in-chain-rule
-  (equal (update-erl-state->in (update-erl-state->in s v1) v2)
-         (update-erl-state->in s v2))
-  :enable (update-erl-state->in))
-
-
-; TODO: ask mark how to generalize these
-(defrule update-lookup-crock
-  (equal (omap::lookup s (omap::update s x m)) x)
-    :enable omap::lookup)
-
-(defrule update-lookup-crock-2
-  (implies 
-    (not (equal s1 s2))
-    (equal (omap::lookup s2 (omap::update s1 x1 (omap::update s2 x2 m))) x2))
-    :enable omap::lookup)
-
-(defrule additional-update-crock
-  (equal (update-erl-state->in (update-erl-state->bind s b) in)
-         (update-erl-state->bind (update-erl-state->in s in) b))
-  :enable (update-erl-state->in update-erl-state->bind))
-
-; TODO: generalize?
-(defrule even-more-crock-lemmas-1
-  (implies (and (erl-val-p x)
-                (equal (erl-val-kind x) :integer)
-                (equal (erl-val-integer->val x) 0))
-           (equal x '(:integer 0)))
-  :enable (erl-val-kind erl-val-integer->val erl-val-p)
-  :expand (TRUE-LISTP (CDR X))
-  :rule-classes :forward-chaining)
-
-(defrule update-erl-state-bind-chain-rule
-  (equal (update-erl-state->bind (update-erl-state->bind s b1) b2)
-         (update-erl-state->bind s b2))
-  :enable (update-erl-state->bind))
-
-(defrule eval-clauses-of-sum-base-case
-  (implies
-    (and (wf-state-p s)
-         (equal (erl-state->world s) (test-w))
-         (equal (erl-state->module s) 'local)
-         
-         ; TODO: ask mark how to simplify this
-         (erl-vlst-p args)
-         (car args)
-         (not (cdr args))
-         (equal (erl-val-kind (car args)) :integer)
-         (equal (erl-val-integer->val (car args)) 0))
-    (equal (eval-clauses
-             args
-             '(((cases (:integer 0))
-                (guards)
-                (body (:integer 0)))
-               ((cases (:var X))
-                (guards ((:call is_integer (:cons (:var X) (:nil))) 
-                        (:binop > (:var X) (:integer 0))))
-                (body (:binop 
-                        + 
-                        (:var X) 
-                        (:call 
-                          sum 
-                          (:cons (:binop - (:var X) (:integer 1)) 
-                                (:nil)))))))
-                  (update-erl-state->bind s nil))
-            (mv (update-erl-state->bind
-                 (update-erl-state->in s (car args))
-                 nil)
-                (list (make-erl-val-integer :val 0)))))
-  :enable 
-    (eval-clauses
-     eval-clauses-when-consp
-     match-args
-     eval-match
-     eval-guard-seq
-     EVAL-GUARD-SEQ-WHEN-CONSP
-     EVAL-GUARD
-     EVAL-GUARD-EXPR
-     eval-bif
-     apply-erl-binop
-     apply-erl-comp-binop
-     erl-compare)
-  :do-not-induct t)
-
-(defrule eval-clauses-of-sum-inductive-step
-  (implies
-    (and (wf-state-p s)
-         (equal (erl-state->world s) (test-w))
-         (equal (erl-state->module s) 'local)
-         
-         ; TODO: ask mark how to simplify this
-         (erl-vlst-p args)
-         (car args)
-         (not (cdr args))
-         (equal (erl-val-kind (car args)) :integer)
-         (> (erl-val-integer->val (car args)) 0))
-    (equal (eval-clauses
-             args
-             '(((cases (:integer 0))
-                (guards)
-                (body (:integer 0)))
-               ((cases (:var X))
-                (guards ((:call is_integer (:cons (:var X) (:nil))) 
-                        (:binop > (:var X) (:integer 0))))
-                (body (:binop 
-                        + 
-                        (:var X) 
-                        (:call 
-                          sum 
-                          (:cons (:binop - (:var X) (:integer 1)) 
-                                (:nil)))))))
-                  (update-erl-state->bind s nil))
-           (mv (update-erl-state->bind
-                 (update-erl-state->in s (car args))
-                 (omap::update 'X (car args) nil))
-               '((:binop 
-                  + 
-                  (:var X) 
-                  (:call 
-                    sum 
-                    (:cons (:binop - (:var X) (:integer 1)) 
-                          (:nil))))))))
-  :enable 
-    (eval-clauses
-     eval-clauses-when-consp
-     match-args
-     eval-match
-     eval-guard-seq
-     EVAL-GUARD-SEQ-WHEN-CONSP
-     EVAL-GUARD
-     EVAL-GUARD-EXPR
-     eval-bif
-     apply-erl-binop
-     apply-erl-comp-binop
-     erl-compare)
-  :do-not-induct t)
-
-(defrule eval-clauses-of-sum-negative
-  (implies
-    (and (wf-state-p s)
-         (equal (erl-state->world s) (test-w))
-         (equal (erl-state->module s) 'local)
-         
-         ; TODO: ask mark how to simplify this
-         (erl-vlst-p args)
-         (car args)
-         (not (cdr args))
-         (equal (erl-val-kind (car args)) :integer)
-         (< (erl-val-integer->val (car args)) 0))
-    (equal (eval-clauses
-             args
-             '(((cases (:integer 0))
-                (guards)
-                (body (:integer 0)))
-               ((cases (:var X))
-                (guards ((:call is_integer (:cons (:var X) (:nil))) 
-                        (:binop > (:var X) (:integer 0))))
-                (body (:binop 
-                        + 
-                        (:var X) 
-                        (:call 
-                          sum 
-                          (:cons (:binop - (:var X) (:integer 1)) 
-                                (:nil)))))))
-                  (update-erl-state->bind s nil))
-           (mv (update-erl-state->bind s nil) nil)))
-  :enable 
-    (eval-clauses
-     eval-clauses-when-consp
-     match-args
-     eval-match
-     eval-guard-seq
-     EVAL-GUARD-SEQ-WHEN-CONSP
-     EVAL-GUARD
-     EVAL-GUARD-EXPR
-     eval-bif
-     apply-erl-binop
-     apply-erl-comp-binop
-     erl-compare)
-  :do-not-induct t)
-
-
-(defrule local-call-of-sum-base-case
-  (implies
-    (and (wf-state-p s)
-         (equal (erl-state->world s) (test-w))
-         (equal (erl-state->module s) 'local)
-         (erl-vlst-p args)
-         (car args)
-         (not (cdr args))
-         (equal (erl-val-kind (car args)) :integer)
-         (equal (erl-val-integer->val (car args)) 0))
-    (equal (eval-local-call s 'sum args)
-           (mv (update-erl-state->bind
-                 (update-erl-state->in s (car args))
-                 nil)
-               '((:integer 0)))))
-    :enable eval-local-call)
-
-(defrule local-call-of-sum-base-inductive
-  (implies
-    (and (wf-state-p s)
-         (equal (erl-state->world s) (test-w))
-         (equal (erl-state->module s) 'local)
-         (erl-vlst-p args)
-         (car args)
-         (not (cdr args))
-         (equal (erl-val-kind (car args)) :integer)
-         (> (erl-val-integer->val (car args)) 0))
-    (equal (eval-local-call s 'sum args)
-           (mv (update-erl-state->bind
-                 (update-erl-state->in s (car args))
-                 (omap::update 'X (car args) nil))
-               '((:binop 
-                  + 
-                  (:var X) 
-                  (:call 
-                    sum 
-                    (:cons (:binop - (:var X) (:integer 1)) 
-                          (:nil))))))))
-    :enable eval-local-call)
-
+; While it is not necessary to admit the theorem below, this lemma speeds up 
+; the proof quite a bit. ACL2 has an easier time dealing with the cases of 
+; eval-local-call and apply-k separately.
 (defrule local-call-of-sum
   (implies
-    (and (wf-state-p s)
-         (equal (erl-state->world s) (test-w))
-         (equal (erl-state->module s) 'local)
-         (erl-vlst-p args)
-         (car args)
-         (not (cdr args))
-         (equal (erl-val-kind (car args)) :integer))
-    (equal (eval-local-call s 'sum args)
-           (if (> (erl-val-integer->val (car args)) 0)
-               (mv (update-erl-state->bind
-                     (update-erl-state->in s (car args))
-                     (omap::update 'X (car args) nil))
-                   '((:binop 
-                       + 
-                       (:var X) 
-                       (:call 
-                          sum 
-                          (:cons (:binop - (:var X) (:integer 1)) 
-                                 (:nil))))))
-               (if (equal (erl-val-integer->val (car args)) 0)
-                   (mv (update-erl-state->bind
-                          (update-erl-state->in s (car args))
-                          nil)
-                        '((:integer 0)))
-                    (mv (update-erl-state->in 
-                          s 
-                          (make-erl-val-excpt 
-                            :err
-                              (make-erl-err
-                                :class (make-err-class-error)
-                                :reason (make-exit-reason-function-clause)))) 
-                        nil)))))
-    :enable eval-local-call)
-
-(include-book "../../theorems/kont-step/local-call")
-(include-book "../../theorems/kont-step/functions")
-(include-book "../../theorems/kont-step/exprs")
-(include-book "../../theorems/kont-step/binop")
-(include-book "../../theorems/kont-step/atomic")
-
-; (defrule lemma-apply-erl-binop
-;   (implies 
-;     (and (erl-val-p left)
-;          (erl-val-p right)
-;          (equal (erl-val-kind left) :integer)
-;          (equal (erl-val-kind right) :integer))
-;     (equal (apply-erl-binop '+ left right)
-;            (make-erl-val-integer 
-;             :val (+ (erl-val-integer->val left)
-;                     (erl-val-integer->val right)))))
-;   :enable (apply-erl-binop apply-erl-arithm-binop erl-add))
-
-(defrule the-great-type-lemma
-  (implies 
     (and 
       (wf-state-p s)
-      (erl-k-p k)
-      (equal (erl-state->world s) (test-w))
+      (equal (erl-state->world s) (sum-test-w))
       (equal (erl-state->module s) 'local)
-      (equal (kont-kind (erl-k->kont k)) :local-call)
-      (equal (kont-local-call->call (erl-k->kont k)) 'sum)
-      (equal (erl-val-kind (erl-state->in s)) :cons)
-      (car (erl-val-cons->lst (erl-state->in s)))
-      (not (cdr (erl-val-cons->lst (erl-state->in s))))
-      (equal (erl-val-kind (car (erl-val-cons->lst (erl-state->in s))))
-             :integer)
-      (>= (erl-val-integer->val (car (erl-val-cons->lst (erl-state->in s)))) 0)
-      (wf-state-p (apply-k s (cons k nil))))
-    (equal (erl-val-kind (erl-state->in (apply-k s (cons k nil)))) :integer))
-  :disable (eval-k-of-local-call->s eval-k-of-local-call->klst)
-  :enable (apply-erl-binop apply-erl-arithm-binop erl-add)
-  :expand (EVAL-K K S))
+      (erl-vlst-p args)
+      (car args)
+      (not (cdr args))
+      (equal (erl-val-kind (car args)) :integer))
+    (equal 
+      (eval-local-call s 'sum args)
+      (if (> (erl-val-integer->val (car args)) 0)
+          (mv (update-erl-state->bind
+                (update-erl-state->in s (car args))
+                (omap::update 'X (car args) nil))
+              '((:binop 
+                  + 
+                  (:var X) 
+                  (:call 
+                    sum 
+                    (:cons (:binop - (:var X) (:integer 1)) 
+                            (:nil))))))
+          (if (equal (erl-val-integer->val (car args)) 0)
+              (mv (update-erl-state->bind
+                    (update-erl-state->in s (car args))
+                    nil)
+                  '((:integer 0)))
+              (mv (update-erl-state->in 
+                    s 
+                    (make-erl-val-excpt 
+                      :err
+                        (make-erl-err
+                          :class (make-err-class-error)
+                          :reason (make-exit-reason-function-clause)))) 
+                  nil)))))
+  :enable
+    (eval-local-call eval-clauses eval-clauses-when-consp
+     match-args eval-match eval-guard-seq eval-guard-seq-when-consp
+     eval-guard eval-guard-expr eval-bif apply-erl-binop
+     apply-erl-comp-binop erl-compare))
 
 
-; THis is the path for when > 0
+; Disable useless runes for efficiency.
+(local 
+  (in-theory (disable 
+    erl-k-p-when-member-equal-of-erl-klst-p erl-val-fix-when-none
+    erl-val-fix-when-flimit default-<-2 default-<-1 default-+-2
+    default-+-1 erl-val-p-when-member-equal-of-erl-vlst-p
+    erl-klst-p-when-subsetp-equal erl-val-p-when-erl-fun-p-rewrite
+    erl-val-p-when-erl-fun-p-rewrite apply-k-of-reject apply-k-of-flimit
+    apply-k-of-excpt)))
 
-
-(in-theory (disable eval-k-of-local-call->s eval-k-of-local-call->klst))
-(include-book "../../theorems/kont-step/cons")
-
-(defrule chain-of-in-bind
-  (equal (update-erl-state->in-bind (update-erl-state->in-bind s v1 b1) v2 b2)
-             (update-erl-state->in-bind s v2 b2))
-  :enable update-erl-state->in-bind)
-
-(defrule in-bind-of-in
-  (equal (update-erl-state->in-bind (update-erl-state->in s v1) v2 b2)
-             (update-erl-state->in-bind s v2 b2))
-  :enable (update-erl-state->in update-erl-state->in-bind))
-
-(defrule in-bind-of-bind
-  (equal (update-erl-state->in-bind (update-erl-state->bind s b1) v2 b2)
-             (update-erl-state->in-bind s v2 b2))
-  :enable (update-erl-state->bind update-erl-state->in-bind))
-
-
-(include-book "std/omaps/top" :dir :system)
-
-(defrule update*-dup
-  (implies (omap::mapp map) (equal (omap::update* map map) map)))
-
-
-(in-theory
-  (disable 
-    ERL-K-P-WHEN-MEMBER-EQUAL-OF-ERL-KLST-P
-    EVAL-K-OF-CONS-MERGE-NONCONS->S
-    EVAL-K-OF-CONS-MERGE-CONS-INCOMPATIBLE->S
-    EVAL-K-OF-CONS-MERGE-CONS-COMPATIBLE->S
-    ERL-VAL-FIX-WHEN-NONE
-    ERL-VAL-FIX-WHEN-FLIMIT
-    DEFAULT-<-2
-    DEFAULT-<-1
-    DEFAULT-+-2
-    DEFAULT-+-1
-    ERL-VAL-P-WHEN-MEMBER-EQUAL-OF-ERL-VLST-P
-    ERL-KLST-P-WHEN-SUBSETP-EQUAL
-    ERL-VAL-P-WHEN-ERL-FUN-P-REWRITE
-    ERL-VAL-P-WHEN-ERL-FUN-P-REWRITE
-    APPLY-K-OF-REJECT
-    APPLY-K-OF-FLIMIT
-    APPLY-K-OF-EXCPT))
-
-(set-case-split-limitations '(5 4))
-
-; runs faster when given fuel > 10
-(defrule the-great-lemma-1
+; Base case of calling apply-k with sum
+(defrule apply-k-of-sum-base-case
   (implies 
     (and
       (wf-state-p s)
       (erl-k-p k)
       (wf-state-p (apply-k s (cons k nil)))
-      (equal (erl-state->world s) (test-w))
+      (equal (erl-state->world s) (sum-test-w))
       (equal (erl-state->module s) 'local)
       (equal (kont-kind (erl-k->kont k)) :local-call)
       (equal (kont-local-call->call (erl-k->kont k)) 'sum)
       (equal (erl-val-kind (erl-state->in s)) :cons)
       (car (erl-val-cons->lst (erl-state->in s)))
       (not (cdr (erl-val-cons->lst (erl-state->in s))))
-      (equal (erl-val-kind (car (erl-val-cons->lst (erl-state->in s))))
-             :integer)
-      (> (erl-val-integer->val (car (erl-val-cons->lst (erl-state->in s)))) 0)
-      (equal (erl-val-kind (erl-state->in (apply-k s (cons k nil)))) :integer))
-    (equal
-      (erl-state->in (apply-k s (cons k nil)))
-      (erl-add
-        (CAR (ERL-VAL-CONS->LST (ERL-STATE->IN S)))
-        (erl-state->in
-          (apply-k 
-            (update-erl-state->in-bind
-              s
-              (erl-val-cons
-                (list (erl-val-integer
-                        (+ -1 
-                          (erl-val-integer->val 
-                            (car (erl-val-cons->lst (erl-state->in s))))))))
-              (omap::update 
-                'x
-                (car (erl-val-cons->lst (erl-state->in s)))
-                nil))
-            (list (ERL-K (+ -5 (ERL-K->FUEL K))
-                '(:LOCAL-CALL SUM)))
-            )))))
-:expand (eval-k k s)
-:do-not-induct t
-:enable (apply-erl-binop APPLY-ERL-ARITHM-BINOP erl-sub erl-add))
-
-(defrule the-great-lemma-2
-  (implies 
-    (and
-      (wf-state-p s)
-      (erl-k-p k)
-      (wf-state-p (apply-k s (cons k nil)))
-      (equal (erl-state->world s) (test-w))
-      (equal (erl-state->module s) 'local)
-      (equal (kont-kind (erl-k->kont k)) :local-call)
-      (equal (kont-local-call->call (erl-k->kont k)) 'sum)
-      (equal (erl-val-kind (erl-state->in s)) :cons)
-      (car (erl-val-cons->lst (erl-state->in s)))
-      (not (cdr (erl-val-cons->lst (erl-state->in s))))
-      (equal (erl-val-kind (car (erl-val-cons->lst (erl-state->in s))))
-             :integer)
-      (= (erl-val-integer->val (car (erl-val-cons->lst (erl-state->in s)))) 0)
-      (equal (erl-val-kind (erl-state->in (apply-k s (cons k nil)))) :integer))
+      (equal (erl-val-kind (car (erl-val-cons->lst (erl-state->in s)))) :integer)
+      (equal (erl-val-kind (erl-state->in (apply-k s (cons k nil)))) :integer)
+      (equal (erl-val-integer->val (car (erl-val-cons->lst (erl-state->in s)))) 0))
     (equal
       (erl-state->in (apply-k s (cons k nil)))
       (make-erl-val-integer :val 0)))
 :expand (eval-k k s)
-:do-not-induct t
-:enable (apply-erl-binop APPLY-ERL-ARITHM-BINOP erl-sub erl-add))
+:enable (apply-erl-binop apply-erl-arithm-binop erl-sub erl-add))
 
-(set-induction-depth-limit 1)
-(define sum-n ((n natp))
-  (b* ((n (nfix n))
-       ((if (= n 0)) 0))
-      (+ n (sum-n (1- n)))))
-
-
-(define crock-induct (args k)
-  (declare (irrelevant k))
-  :verify-guards nil
-  :enabled t
-  :measure (nfix (erl-val-integer->val (car (erl-val-cons->lst (erl-state->in args)))))
-  (if (< (erl-val-integer->val (car (erl-val-cons->lst (erl-state->in args)))) 0)
-      nil
-      (if (= (erl-val-integer->val (car (erl-val-cons->lst (erl-state->in args)))) 0)
-          t
-          (crock-induct
-            (update-erl-state->in-bind
-              args
-              (erl-val-cons
-                (list (erl-val-integer
-                        (+ -1 
-                          (erl-val-integer->val 
-                            (car (erl-val-cons->lst (erl-state->in args))))))))
-              (omap::update 
-                'x
-                (car (erl-val-cons->lst (erl-state->in args)))
-                nil))
-            (ERL-K (+ -5 (erl-k->fuel k))
-                '(:LOCAL-CALL SUM))))))
-
-
-(defrule the-great-lemma-3
+; Inductive step of calling apply-k with sum
+(defrule apply-k-of-sum-inductive-step
   (implies 
     (and
       (wf-state-p s)
       (erl-k-p k)
       (wf-state-p (apply-k s (cons k nil)))
-      (equal (erl-state->world s) (test-w))
+      (equal (erl-state->world s) (sum-test-w))
       (equal (erl-state->module s) 'local)
       (equal (kont-kind (erl-k->kont k)) :local-call)
       (equal (kont-local-call->call (erl-k->kont k)) 'sum)
       (equal (erl-val-kind (erl-state->in s)) :cons)
       (car (erl-val-cons->lst (erl-state->in s)))
       (not (cdr (erl-val-cons->lst (erl-state->in s))))
-      (equal (erl-val-kind (car (erl-val-cons->lst (erl-state->in s))))
-             :integer)
-      (> (erl-val-integer->val (car (erl-val-cons->lst (erl-state->in s)))) 0)
-      (equal (erl-val-kind (erl-state->in (apply-k s (cons k nil)))) :integer))
+      (equal (erl-val-kind (car (erl-val-cons->lst (erl-state->in s)))) :integer)
+      (equal (erl-val-kind (erl-state->in (apply-k s (cons k nil)))) :integer)
+      (> (erl-val-integer->val (car (erl-val-cons->lst (erl-state->in s)))) 0))
     (equal
-      (erl-val-kind 
+      (erl-state->in (apply-k s (cons k nil)))
+      (erl-add
+        (car (erl-val-cons->lst (erl-state->in s)))
         (erl-state->in
           (apply-k 
-            (update-erl-state->in-bind
-              s
-              (erl-val-cons
-                (list (erl-val-integer
+            (update-erl-state->bind
+              (update-erl-state->in
+                s
+                (erl-val-cons
+                  (list 
+                    (erl-val-integer
                       (+ -1 
                         (erl-val-integer->val 
-                          (car (erl-val-cons->lst (erl-state->in s))))))))
+                            (car (erl-val-cons->lst (erl-state->in s)))))))))
               (omap::update 
-                'x
+                'X
                 (car (erl-val-cons->lst (erl-state->in s)))
                 nil))
-            (list (ERL-K (+ -5 (ERL-K->FUEL K))
-                '(:LOCAL-CALL SUM))))))
-    :integer))
-  :use (:instance the-great-lemma-1)
-  :enable erl-add)
+            (list (erl-k (+ -5 (erl-k->fuel k))
+                         '(:local-call sum)))
+            )))))
+:expand (eval-k k s)
+:enable (apply-erl-binop apply-erl-arithm-binop erl-sub erl-add)
+:disable (eval-k-of-local-call->s eval-k-of-local-call->klst)
+:case-split-limitations (5 1))
 
-
-
-(defrule the-great-induction
+; Remark: This is a rule I added after realizing ACL2 forgets that the returned
+; erl-state should be well-formed after applying the rewrite rule above. This 
+; lemma should trivially follow from apply-k-of-sum-inductive-step, but I will
+; keep it in for now, until I figure out why it is not obvious to ACL2.
+(defrule apply-k-of-sum-inductive-step-wf
   (implies 
     (and
       (wf-state-p s)
       (erl-k-p k)
-      (equal (erl-state->world s) (test-w))
+      (wf-state-p (apply-k s (cons k nil)))
+      (equal (erl-state->world s) (sum-test-w))
       (equal (erl-state->module s) 'local)
       (equal (kont-kind (erl-k->kont k)) :local-call)
       (equal (kont-local-call->call (erl-k->kont k)) 'sum)
       (equal (erl-val-kind (erl-state->in s)) :cons)
       (car (erl-val-cons->lst (erl-state->in s)))
       (not (cdr (erl-val-cons->lst (erl-state->in s))))
-      (equal (erl-val-kind (car (erl-val-cons->lst (erl-state->in s))))
-             :integer)
+      (equal (erl-val-kind (car (erl-val-cons->lst (erl-state->in s)))) :integer)
+      (equal (erl-val-kind (erl-state->in (apply-k s (cons k nil)))) :integer)
+      (> (erl-val-integer->val (car (erl-val-cons->lst (erl-state->in s)))) 0))
+    (equal
+      (erl-val-kind 
+        (erl-state->in
+          (apply-k 
+            (update-erl-state->bind
+              (update-erl-state->in s
+                (erl-val-cons
+                  (list
+                    (erl-val-integer
+                      (+ -1 
+                         (erl-val-integer->val 
+                           (car (erl-val-cons->lst (erl-state->in s)))))))))
+              (omap::update 
+                'x
+                (car (erl-val-cons->lst (erl-state->in s)))
+                nil))
+            (list (erl-k (+ -5 (erl-k->fuel k))
+                         '(:local-call sum))))))
+    :integer))
+  :use (:instance apply-k-of-sum-inductive-step)
+  :enable erl-add
+  :disable (eval-k-of-local-call->s eval-k-of-local-call->klst))
+
+; This theorem later allows erl-val-integer->val to be called on the result
+; of (apply-k s (cons k nil)) without needing to expand more terms.
+(defrule val-kind-of-apply-k-of-sum
+  (implies 
+    (and 
+      (wf-state-p s)
+      (erl-k-p k)
+      (equal (erl-state->world s) (sum-test-w))
+      (equal (erl-state->module s) 'local)
+      (equal (kont-kind (erl-k->kont k)) :local-call)
+      (equal (kont-local-call->call (erl-k->kont k)) 'sum)
+      (equal (erl-val-kind (erl-state->in s)) :cons)
+      (car (erl-val-cons->lst (erl-state->in s)))
+      (not (cdr (erl-val-cons->lst (erl-state->in s))))
+      (equal (erl-val-kind (car (erl-val-cons->lst (erl-state->in s)))) :integer)
       (>= (erl-val-integer->val (car (erl-val-cons->lst (erl-state->in s)))) 0)
       (wf-state-p (apply-k s (cons k nil))))
+    (equal (erl-val-kind (erl-state->in (apply-k s (cons k nil)))) :integer))
+  :expand (eval-k k s)
+  :enable (apply-erl-binop apply-erl-arithm-binop erl-add)
+  :disable (eval-k-of-local-call->s eval-k-of-local-call->klst)
+  :case-split-limitations (5 1))
+
+; Induction schema for apply-k-of-sum
+(local (define apply-k-of-sum-induct (args k)
+  (declare (irrelevant k))
+  :measure 
+    (nfix 
+      (erl-val-integer->val 
+        (car (erl-val-cons->lst (erl-state->in args)))))
+  :verify-guards nil
+  :enabled t
+  (if (< (erl-val-integer->val 
+            (car (erl-val-cons->lst (erl-state->in args)))) 0)
+      nil
+      (if (= (erl-val-integer->val 
+                (car (erl-val-cons->lst (erl-state->in args)))) 0)
+          t
+          (apply-k-of-sum-induct
+            (update-erl-state->in-bind
+              args
+              (erl-val-cons
+                (list 
+                  (erl-val-integer
+                    (+ -1 
+                       (erl-val-integer->val 
+                         (car (erl-val-cons->lst (erl-state->in args))))))))
+              (omap::update 
+                'X
+                (car (erl-val-cons->lst (erl-state->in args)))
+                nil))
+            (erl-k (+ -5 (erl-k->fuel k))
+                   '(:local-call sum)))))))
+
+; apply-k-of-sum is equivalent to the lisp sum.
+(defrule apply-k-of-sum-kont
+  (implies 
+    (and
+      (wf-state-p s)
+      (erl-k-p k)
+      (equal (erl-state->world s) (sum-test-w))
+      (equal (erl-state->module s) 'local)
+      (equal (kont-kind (erl-k->kont k)) :local-call)
+      (equal (kont-local-call->call (erl-k->kont k)) 'sum)
+      (equal (erl-val-kind (erl-state->in s)) :cons)
+      (car (erl-val-cons->lst (erl-state->in s)))
+      (not (cdr (erl-val-cons->lst (erl-state->in s))))
+      (equal (erl-val-kind (car (erl-val-cons->lst (erl-state->in s)))) :integer)
+      (wf-state-p (apply-k s (cons k nil)))
+      (>= (erl-val-integer->val (car (erl-val-cons->lst (erl-state->in s)))) 0))
     (equal
       (erl-state->in (apply-k s (cons k nil)))
       (make-erl-val-integer 
         :val
-          (sum-n (erl-val-integer->val (car (erl-val-cons->lst (erl-state->in s))))))))
-:induct (crock-induct s k)
-:disable (apply-k-of-step apply-k-of-consp)
-:enable (sum-n erl-add))
+          (sum (erl-val-integer->val 
+                 (car (erl-val-cons->lst (erl-state->in s))))))))
+:induct (apply-k-of-sum-induct s k)
+:enable (sum erl-add)
+:disable (apply-k-of-step apply-k-of-consp))
 
+
+; Remark: I should be able to remove the use hint with some work.
+(defrule apply-k-of-sum
+  (b* (; The starting state is well-formed
+       ((unless (wf-state-p s)) t) 
+       ((erl-state s) s)
+       ((unless (equal s.world (sum-test-w))) t)
+       ((unless (equal s.module 'local)) t)
+       
+       ; The next continuation calls sum(N)
+       ((unless (erl-k-p k)) t)
+       ((erl-k k) k)
+       ((unless (equal (kont-kind k.kont) :expr)) t)
+       ((unless (equal (node-kind (kont-expr->expr k.kont)) :call)) t)
+       ((unless (equal (node-call->fn (kont-expr->expr k.kont)) 'sum)) t)
+
+       ; Result of the function call does not cause an error
+       ((unless (wf-state-p (apply-k s (list k)))) t)
+
+       ; Properties of the function arguments
+       ; Remark: a lot of these can be removed with some work.
+       (args
+        (apply-k
+          (update-erl-state->in s '(:none))
+          (list
+            (make-erl-k
+              :fuel (1- k.fuel)
+              :kont
+                (make-kont-expr
+                  :expr
+                    (node-call->args
+                      (kont-expr->expr k.kont)))))))
+
+       ; TODO: remove this when the apply-k-of-module theorem is complete
+       ; - in ../../theorems/state/module 
+       ((unless (equal (erl-state->module args) 'local)) t)
+
+       ; The argument must evaluate to a list of two integers.
+       ((unless (wf-state-p args)) t)
+       ((unless (equal (erl-val-kind (erl-state->in args)) :cons)) t)
+       (vals (erl-val-cons->lst (erl-state->in args)))
+       ((unless 
+          (and (car vals)
+               (equal (erl-val-kind (car vals)) :integer)
+               (>= (erl-val-integer->val (car vals)) 0)
+               (not (cdr vals)))) t))
+
+    (equal (erl-state->in (apply-k s (cons k nil)))
+           (erl-val-integer (sum (erl-val-integer->val (car vals))))))
+  :disable 
+    (erl-k-p-when-member-equal-of-erl-klst-p default-<-2 default-<-1
+     kont-expr->expr-of-kont-expr expr-fix-is-the-identity-on-expr
+     expr-fix-is-the-identity-on-expr expr-call-ensures
+     return-type-of-kont-expr eval-k-of-local-call->s 
+     eval-k-of-local-call->klst)
+  :case-split-limitations (5 1)
+  :use 
+    (:instance apply-k-of-sum-kont
+      (s (apply-k
+          (update-erl-state->in s '(:none))
+          (list
+            (make-erl-k
+              :fuel (1- (erl-k->fuel k))
+              :kont
+                (make-kont-expr
+                  :expr
+                    (node-call->args
+                      (kont-expr->expr (erl-k->kont k))))))))
+      (k (erl-k (+ -1 (erl-k->fuel k))
+                '(:local-call sum)))))
