acl2/books/arithmetic/top.lisp
@@ -1,0 +1,4 @@
+(in-package "ACL2")
+
+(include-book "add")
+(include-book "sum")
