acl2/theorems/kont-step/case-of.lisp
@@ -1,9 +1,7 @@
 (in-package "ACL2")
 (include-book "../core/eval-theorems")
 
-
 ; Case-of Kont-Step ------------------------------------------------------------
-
 
 ; The following theorems show that evaluating a continuation for a case of
 ; expression is equivalent to evaluating the argument of the case and then
@@ -14,290 +12,147 @@
 (defrule eval-k-of-expr-case-of->klst
   (implies
     (and
-       (wf-state-p s) 
+       (erl-state-p s)
        (erl-k-p k)
-       (> (erl-k->fuel k) 0)
        (equal (kont-kind (erl-k->kont k)) :expr)
        (equal (node-kind (kont-expr->expr (erl-k->kont k))) :case-of))
     (equal
       (erl-s-klst->klst (eval-k k s))
-      (list 
-        (make-erl-k 
-          :fuel (1- (erl-k->fuel k))
-          :kont (make-kont-expr 
-            :expr (node-case-of->expr (kont-expr->expr (erl-k->kont k)))))
-        (make-erl-k 
-          :fuel (1- (erl-k->fuel k))
-          :kont (make-kont-case-of
-            :clauses (node-case-of->clauses (kont-expr->expr (erl-k->kont k))))))))
+      (if (and (wf-state-p s) (> (erl-k->fuel k) 0))
+          (list 
+            (make-erl-k 
+              :fuel (1- (erl-k->fuel k))
+              :kont (make-kont-expr 
+                :expr (node-case-of->expr (kont-expr->expr (erl-k->kont k)))))
+            (make-erl-k 
+              :fuel (1- (erl-k->fuel k))
+              :kont (make-kont-case-of
+                :clauses (node-case-of->clauses (kont-expr->expr (erl-k->kont k))))))
+          nil)))
   :enable eval-k)
 
 (defrule eval-k-of-expr-case-of->s
   (implies
     (and
-       (wf-state-p s) 
+       (erl-state-p s)
        (erl-k-p k)
-       (> (erl-k->fuel k) 0)
        (equal (kont-kind (erl-k->kont k)) :expr)
        (equal (node-kind (kont-expr->expr (erl-k->kont k))) :case-of))
     (equal
-      (erl-s-klst->s (eval-k k s)) (update-erl-state->in s (make-erl-val-none))))
+      (erl-s-klst->s (eval-k k s)) 
+      (cond
+        ((not (wf-state-p s)) s)
+        ((not (> (erl-k->fuel k) 0))
+         (update-erl-state->in s (make-erl-val-flimit)))
+        (t (update-erl-state->in s (make-erl-val-none))))))
   :enable eval-k)
+
 
 ; kont-case-of
-(defrule eval-k-of-case-of-ok->klst
-  (implies
-    (and
-       (wf-state-p s) 
-       (erl-k-p k)
-       (> (erl-k->fuel k) 0)
-       (equal (kont-kind (erl-k->kont k)) :case-of)
-       (not (equal (erl-val-kind (erl-state->in
-                    (mv-nth 
-                      0
-                      (eval-clauses 
-                          (list (erl-state->in s))
-                          (kont-case-of->clauses (erl-k->kont k))
-                          s))))
-                :reject))
-       (mv-nth 1 (eval-clauses 
-                  (list (erl-state->in s))
-                  (kont-case-of->clauses (erl-k->kont k))
-                  s)))
-    (equal
-      (erl-s-klst->klst (eval-k k s))
-      (list 
-        (make-erl-k 
-          :fuel (1- (erl-k->fuel k))
-          :kont (make-kont-expr 
-            :expr (car (mv-nth 
-                          1
-                          (eval-clauses 
-                            (list (erl-state->in s))
-                            (kont-case-of->clauses (erl-k->kont k))
-                            s)))))
-        (make-erl-k 
-          :fuel (1- (erl-k->fuel k))
-          :kont (make-kont-exprs
-            :exprs (cdr (mv-nth 
-                          1
-                          (eval-clauses 
-                            (list (erl-state->in s))
-                            (kont-case-of->clauses (erl-k->kont k))
-                            s))))))))
-  :enable eval-k)
-
-(defrule eval-k-of-case-of-ok->s
-  (implies
-    (and (wf-state-p s) 
-         (erl-k-p k)
-         (> (erl-k->fuel k) 0)
-         (equal (kont-kind (erl-k->kont k)) :case-of)
-         (not (equal (erl-val-kind (erl-state->in
-                       (mv-nth 
-                         0
-                         (eval-clauses 
-                           (list (erl-state->in s))
-                           (kont-case-of->clauses (erl-k->kont k))
-                           s))))
-                     :reject))
-         (mv-nth 1 (eval-clauses 
-                     (list (erl-state->in s))
-                     (kont-case-of->clauses (erl-k->kont k))
-                     s)))
-    (equal (erl-s-klst->s (eval-k k s))
-           (update-erl-state->in
-            (mv-nth 
-              0
-              (eval-clauses 
-                (list (erl-state->in s))
-                (kont-case-of->clauses (erl-k->kont k))
-                s))
-            (make-erl-val-none))))
-  :enable eval-k)
-
-(defrule eval-k-of-case-of-reject->klst
-  (implies
-    (and
-       (wf-state-p s) 
-       (erl-k-p k)
-       (> (erl-k->fuel k) 0)
-       (equal (kont-kind (erl-k->kont k)) :case-of)
-       (equal (erl-val-kind (erl-state->in
-                    (mv-nth 
-                      0
-                      (eval-clauses 
-                          (list (erl-state->in s))
-                          (kont-case-of->clauses (erl-k->kont k))
-                          s))))
-                :reject))
-    (equal (erl-s-klst->klst (eval-k k s)) nil))
-  :enable eval-k)
-
-(defrule eval-k-of-case-of-reject->s
-  (implies
-    (and
-       (wf-state-p s) 
-       (erl-k-p k)
-       (> (erl-k->fuel k) 0)
-       (equal (kont-kind (erl-k->kont k)) :case-of)
-       (equal (erl-val-kind (erl-state->in
-                    (mv-nth 
-                      0
-                      (eval-clauses 
-                          (list (erl-state->in s))
-                          (kont-case-of->clauses (erl-k->kont k))
-                          s))))
-                :reject))
-    (equal (erl-s-klst->s (eval-k k s))
-           (mv-nth 
-             0
-             (eval-clauses 
-               (list (erl-state->in s))
-               (kont-case-of->clauses (erl-k->kont k))
-               s))))
-  :enable eval-k)
-
-(defrule eval-k-of-case-of-no-clauses->klst
-  (implies
-    (and
-       (wf-state-p s) 
-       (erl-k-p k)
-       (> (erl-k->fuel k) 0)
-       (equal (kont-kind (erl-k->kont k)) :case-of)
-       (not (equal (erl-val-kind (erl-state->in
-                    (mv-nth 
-                      0
-                      (eval-clauses 
-                          (list (erl-state->in s))
-                          (kont-case-of->clauses (erl-k->kont k))
-                          s))))
-                :reject))
-       (not (mv-nth 
-              1 (eval-clauses 
-                  (list (erl-state->in s))
-                  (kont-case-of->clauses (erl-k->kont k))
-                  s))))
-    (equal (erl-s-klst->klst (eval-k k s)) nil))
-  :enable eval-k)
-
-(defrule eval-k-of-case-of-no-clauses->s
-  (implies
-    (and
-       (wf-state-p s) 
-       (erl-k-p k)
-       (> (erl-k->fuel k) 0)
-       (equal (kont-kind (erl-k->kont k)) :case-of)
-       (not (equal (erl-val-kind (erl-state->in
-                    (mv-nth 
-                      0
-                      (eval-clauses 
-                          (list (erl-state->in s))
-                          (kont-case-of->clauses (erl-k->kont k))
-                          s))))
-                :reject))
-       (not (mv-nth 
-              1 (eval-clauses 
-                  (list (erl-state->in s))
-                  (kont-case-of->clauses (erl-k->kont k))
-                  s))))
-    (equal (erl-s-klst->s (eval-k k s))
-           (update-erl-state->in 
-            s
-            (make-erl-val-excpt 
-              :err (make-erl-err :class (make-err-class-error)
-                                  :reason (make-exit-reason-case-clause 
-                                            :val (erl-state->in s)))))))
-  :enable eval-k)
-
-
-; Combine the rules from above to a general rewrite rule
 (defrule eval-k-of-case-of->klst
   (implies
     (and
-       (wf-state-p s) 
+       (erl-state-p s)
        (erl-k-p k)
-       (> (erl-k->fuel k) 0)
        (equal (kont-kind (erl-k->kont k)) :case-of))
     (equal
       (erl-s-klst->klst (eval-k k s))
-      (cond 
-        ((equal (erl-val-kind (erl-state->in
-                    (mv-nth 
-                      0
-                      (eval-clauses 
+      (cond
+        ((not (wf-state-p s)) nil)
+        ((not (> (erl-k->fuel k) 0)) nil)
+        ((equal
+           (erl-val-kind
+             (erl-state->in
+               (mv-nth
+                 0
+                 (eval-clauses
+                   (list (erl-state->in s))
+                   (kont-case-of->clauses (erl-k->kont k))
+                   s))))
+           :reject)
+         nil)
+        ((not
+           (mv-nth
+             1
+             (eval-clauses 
+               (list (erl-state->in s))
+               (kont-case-of->clauses (erl-k->kont k))
+               s)))
+         nil)
+        (t (list 
+             (make-erl-k 
+               :fuel (1- (erl-k->fuel k))
+               :kont
+                 (make-kont-expr 
+                  :expr
+                    (car 
+                      (mv-nth 
+                        1
+                        (eval-clauses 
                           (list (erl-state->in s))
                           (kont-case-of->clauses (erl-k->kont k))
-                          s))))
-                :reject)
-          nil)
-        ((not (mv-nth 
-              1 (eval-clauses 
-                  (list (erl-state->in s))
-                  (kont-case-of->clauses (erl-k->kont k))
-                  s)))
-          nil)
-        (t (list 
-            (make-erl-k 
-              :fuel (1- (erl-k->fuel k))
-              :kont (make-kont-expr 
-                :expr (car (mv-nth 
-                              1
-                              (eval-clauses 
-                                (list (erl-state->in s))
-                                (kont-case-of->clauses (erl-k->kont k))
-                                s)))))
-            (make-erl-k 
-              :fuel (1- (erl-k->fuel k))
-              :kont (make-kont-exprs
-                :exprs (cdr (mv-nth 
-                              1
-                              (eval-clauses 
-                                (list (erl-state->in s))
-                                (kont-case-of->clauses (erl-k->kont k))
-                                s))))))))))
+                          s)))))
+             (make-erl-k 
+               :fuel (1- (erl-k->fuel k))
+               :kont
+                 (make-kont-exprs
+                   :exprs
+                     (cdr 
+                       (mv-nth 
+                         1
+                         (eval-clauses 
+                           (list (erl-state->in s))
+                           (kont-case-of->clauses (erl-k->kont k))
+                           s))))))))))
   :enable eval-k)
 
 (defrule eval-k-of-case-of->s
   (implies
     (and
-       (wf-state-p s) 
+       (erl-state-p s) 
        (erl-k-p k)
-       (> (erl-k->fuel k) 0)
        (equal (kont-kind (erl-k->kont k)) :case-of))
     (equal
       (erl-s-klst->s (eval-k k s))
-      (cond 
-        ((equal (erl-val-kind (erl-state->in
-                    (mv-nth 
-                      0
-                      (eval-clauses 
-                          (list (erl-state->in s))
-                          (kont-case-of->clauses (erl-k->kont k))
-                          s))))
-                :reject)
+      (cond
+        ((not (wf-state-p s)) s)
+        ((not (> (erl-k->fuel k) 0))
+         (update-erl-state->in s (make-erl-val-flimit)))
+        ((equal
+           (erl-val-kind
+             (erl-state->in
+               (mv-nth
+                 0
+                 (eval-clauses
+                   (list (erl-state->in s))
+                   (kont-case-of->clauses (erl-k->kont k))
+                   s))))
+           :reject)
+         (mv-nth 
+           0
+           (eval-clauses 
+             (list (erl-state->in s))
+             (kont-case-of->clauses (erl-k->kont k))
+             s)))
+        ((not 
           (mv-nth 
-             0
-             (eval-clauses 
-               (list (erl-state->in s))
-               (kont-case-of->clauses (erl-k->kont k))
-               s)))
-        ((not (mv-nth 
-              1 (eval-clauses 
-                  (list (erl-state->in s))
-                  (kont-case-of->clauses (erl-k->kont k))
-                  s)))
-          (update-erl-state->in 
-            s
-            (make-erl-val-excpt 
-              :err (make-erl-err :class (make-err-class-error)
-                                  :reason (make-exit-reason-case-clause 
-                                            :val (erl-state->in s))))))
+            1 
+            (eval-clauses 
+              (list (erl-state->in s))
+              (kont-case-of->clauses (erl-k->kont k))
+              s)))
+         (update-erl-state->in 
+           s
+           (make-erl-val-excpt 
+             :err (make-erl-err :class (make-err-class-error)
+                                :reason (make-exit-reason-case-clause 
+                                          :val (erl-state->in s))))))
         (t (update-erl-state->in
-            (mv-nth 
-              0
-              (eval-clauses 
-                (list (erl-state->in s))
-                (kont-case-of->clauses (erl-k->kont k))
-                s))
-            (make-erl-val-none)))))))
+             (mv-nth
+               0
+               (eval-clauses
+                 (list (erl-state->in s))
+                 (kont-case-of->clauses (erl-k->kont k))
+                 s))
+             (make-erl-val-none))))))
+  :enable eval-k)
