acl2/theorems/kont-step/cons.lisp
@@ -18,17 +18,20 @@
       (erl-s-klst->klst (eval-k k s))
       (cond 
         ((not (wf-state-p s)) nil)
-        ((not (> (erl-k->fuel k) 0)) nil)
-          
+        ((not (> (erl-k->fuel k) 0)) nil) 
         (t (list 
              (make-erl-k 
               :fuel (1- (erl-k->fuel k))
-              :kont (make-kont-expr :expr 
-                (node-cons->hd (kont-expr->expr (erl-k->kont k)))))
+              :kont 
+                (make-kont-expr 
+                  :expr
+                    (node-cons->hd (kont-expr->expr (erl-k->kont k)))))
              (make-erl-k :fuel (1- (erl-k->fuel k))
                          :kont 
                           (make-kont-cons 
-                            :cdr-expr (node-cons->tl (kont-expr->expr (erl-k->kont k)))
+                            :cdr-expr
+                              (node-cons->tl
+                                (kont-expr->expr (erl-k->kont k)))
                             :bind-0 (erl-state->bind s))))))))
   :enable eval-k)
 
@@ -46,6 +49,7 @@
              (t (update-erl-state->in s (make-erl-val-none))))))
   :enable eval-k)
 
+
 ; kont-cons
 (defrule eval-k-of-cons->klst
   (implies 
@@ -56,8 +60,9 @@
            (if (and (wf-state-p s) (> (erl-k->fuel k) 0))
                (list (make-erl-k 
                       :fuel (1- (erl-k->fuel k)) 
-                      :kont (make-kont-expr 
-                              :expr (kont-cons->cdr-expr (erl-k->kont k))))
+                      :kont
+                        (make-kont-expr 
+                          :expr (kont-cons->cdr-expr (erl-k->kont k))))
                      (make-erl-k 
                       :fuel (1- (erl-k->fuel k))
                       :kont (make-kont-cons-merge 
@@ -82,6 +87,7 @@
                   (kont-cons->bind-0 (erl-k->kont k)))))))
   :enable eval-k)
 
+
 ; kont-cons-merge
 (defrule eval-k-of-cons-merge->klst
   (implies
@@ -91,64 +97,6 @@
     (equal (erl-s-klst->klst (eval-k k s)) nil))
   :enable eval-k)
 
-(defrule eval-k-of-cons-merge-cons-compatible->s
-  (implies
-    (and (wf-state-p s)
-         (erl-k-p k)
-         (> (erl-k->fuel k) 0)
-         (equal (kont-kind (erl-k->kont k)) :cons-merge)
-         (equal (erl-val-kind (erl-state->in s)) :cons)
-         (omap::compatiblep (erl-state->bind s)
-                            (kont-cons-merge->car-bind (erl-k->kont k))))
-    (equal
-      (erl-s-klst->s (eval-k k s))
-      (update-erl-state->in-bind
-        s
-        (make-erl-val-cons
-          :lst (cons (kont-cons-merge->car-val (erl-k->kont k))
-                     (erl-val-cons->lst (erl-state->in s))))
-        (omap::update*
-          (erl-state->bind s)
-          (kont-cons-merge->car-bind (erl-k->kont k))))))
-  :enable eval-k)
-
-(defrule eval-k-of-cons-merge-cons-incompatible->s
-  (implies
-    (and (wf-state-p s)
-         (erl-k-p k)
-         (> (erl-k->fuel k) 0)
-         (equal (kont-kind (erl-k->kont k)) :cons-merge)
-         (equal (erl-val-kind (erl-state->in s)) :cons)
-         (not (omap::compatiblep (erl-state->bind s)
-                                 (kont-cons-merge->car-bind (erl-k->kont k)))))
-    (equal
-      (erl-s-klst->s (eval-k k s))
-      (update-erl-state->in
-        s
-        (make-erl-val-excpt
-          :err (make-erl-err
-                 :class (make-err-class-error)
-                 :reason (make-exit-reason-badmatch
-                           :val (erl-state->in s)))))))
-  :enable eval-k)
-
-(defrule eval-k-of-cons-merge-noncons->s
-  (implies
-    (and (wf-state-p s)
-         (erl-k-p k)
-         (> (erl-k->fuel k) 0)
-         (equal (kont-kind (erl-k->kont k)) :cons-merge)
-         (not (equal (erl-val-kind (erl-state->in s)) :cons)))
-    (equal
-      (erl-s-klst->s (eval-k k s))
-      (update-erl-state->in
-        s
-        (make-erl-val-reject
-          :err "cons-merge expects list, pairs are not supported"))))
-  :enable eval-k)
-
-
-; Combine to general rule
 (defrule eval-k-of-cons-merge->s
   (implies
     (and (erl-state-p s)
@@ -165,16 +113,17 @@
            s
            (make-erl-val-reject
              :err "cons-merge expects list, pairs are not supported")))
-        ((not (omap::compatiblep 
+        ((not 
+          (omap::compatiblep
             (erl-state->bind s)
             (kont-cons-merge->car-bind (erl-k->kont k))))
          (update-erl-state->in
-          s
-          (make-erl-val-excpt
-            :err (make-erl-err
-                  :class (make-err-class-error)
-                   :reason (make-exit-reason-badmatch
-                             :val (erl-state->in s))))))
+           s
+           (make-erl-val-excpt
+             :err (make-erl-err
+                    :class (make-err-class-error)
+                    :reason (make-exit-reason-badmatch
+                              :val (erl-state->in s))))))
         (t (update-erl-state->in-bind
              s
              (make-erl-val-cons
