acl2/theorems/kont-step/exprs.lisp
@@ -1,8 +1,7 @@
 (in-package "ACL2")
 (include-book "../core/eval-theorems")
 
-
-; Kont-Step for Consequitve Expression -----------------------------------------
+; Kont-Step for Consequitve Expressions ----------------------------------------
 
 (defrule eval-k-exprs->s
   (implies
@@ -24,10 +23,14 @@
       (erl-s-klst->klst (eval-k k s))
         (list (make-erl-k 
                 :fuel (1- (erl-k->fuel k))
-                :kont (make-kont-expr :expr (car (kont-exprs->exprs (erl-k->kont k)))))
+                :kont
+                  (make-kont-expr 
+                    :expr (car (kont-exprs->exprs (erl-k->kont k)))))
               (make-erl-k
                 :fuel (1- (erl-k->fuel k))
-                :kont (make-kont-exprs :exprs (cdr (kont-exprs->exprs (erl-k->kont k))))))))
+                :kont
+                  (make-kont-exprs
+                    :exprs (cdr (kont-exprs->exprs (erl-k->kont k))))))))
   :enable eval-k)
 
 (defrule eval-k-exprs-nil->klst
@@ -39,56 +42,3 @@
          (null (kont-exprs->exprs (erl-k->kont k))))
     (equal (erl-s-klst->klst (eval-k k s)) nil))
   :enable eval-k)
-
-; Combined
-; (defrule eval-k-exprs->klst-no-constraints
-;   (implies
-;     (and (erl-state-p s)
-;          (> (erl-k->fuel k) 0)
-;          (erl-k-p k)
-;          (equal (kont-kind (erl-k->kont k)) :exprs))
-;     (equal
-;       (erl-s-klst->klst (eval-k k s))
-;       (cond
-;         ((not (wf-state-p s)) nil)
-;         ((not (> (erl-k->fuel k) 0)) nil)
-;         ((null (kont-exprs->exprs (erl-k->kont k))) nil)
-;         (t (list (make-erl-k 
-;                   :fuel (1- (erl-k->fuel k))
-;                   :kont (make-kont-expr :expr (car (kont-exprs->exprs (erl-k->kont k)))))
-;                  (make-erl-k
-;                   :fuel (1- (erl-k->fuel k))
-;                   :kont (make-kont-exprs :exprs (cdr (kont-exprs->exprs (erl-k->kont k))))))))))
-;   :enable eval-k)
-
-; (defrule eval-k-exprs->klst
-;   (implies
-;     (and (erl-state-p s)
-;          (erl-k-p k)
-;          (equal (kont-kind (erl-k->kont k)) :exprs))
-;     (equal
-;       (erl-s-klst->klst (eval-k k s))
-;       (cond
-;         ((not (wf-state-p s)) nil)
-;         ((not (> (erl-k->fuel k) 0)) nil)
-;         ((null (kont-exprs->exprs (erl-k->kont k))) nil)
-;         (t (list (make-erl-k 
-;                   :fuel (1- (erl-k->fuel k))
-;                   :kont (make-kont-expr :expr (car (kont-exprs->exprs (erl-k->kont k)))))
-;                  (make-erl-k
-;                   :fuel (1- (erl-k->fuel k))
-;                   :kont (make-kont-exprs :exprs (cdr (kont-exprs->exprs (erl-k->kont k))))))))))
-;   :enable eval-k)
-
-; (defrule eval-k-exprs->s
-;   (implies
-;     (and (erl-state-p s)
-;          (erl-k-p k)
-;          (equal (kont-kind (erl-k->kont k)) :exprs))
-;     (equal (erl-s-klst->s (eval-k k s))
-;            (cond
-;             ((not (wf-state-p s)) s)
-;             ((not (> (erl-k->fuel k) 0))
-;              (update-erl-state->in s (make-erl-val-flimit)))
-;             (t s))))
-;   :enable eval-k)
