acl2/theorems/kont-step/fun-call.lisp
@@ -10,108 +10,53 @@
 ; expr-fun-call
 (defrule eval-k-of-expr-fun-call->klst
   (implies
-    (and (wf-state-p s)
+    (and (erl-state-p s)
          (erl-k-p k)
-         (> (erl-k->fuel k) 0)
          (equal (kont-kind (erl-k->kont k)) :expr)
          (equal (node-kind (kont-expr->expr (erl-k->kont k))) :fun-call))
     (equal
       (erl-s-klst->klst (eval-k k s))
-      (list
-        (make-erl-k
-          :fuel (1- (erl-k->fuel k))
-          :kont (make-kont-expr
-                  :expr (node-fun-call->fun
-                           (kont-expr->expr (erl-k->kont k)))))
-        (make-erl-k
-          :fuel (1- (erl-k->fuel k))
-          :kont (make-kont-fun-call-args
-                  :args (node-fun-call->args
-                          (kont-expr->expr (erl-k->kont k))))))))
+      (if (and (wf-state-p s) (> (erl-k->fuel k) 0))
+          (list
+            (make-erl-k
+              :fuel (1- (erl-k->fuel k))
+              :kont (make-kont-expr
+                      :expr (node-fun-call->fun
+                              (kont-expr->expr (erl-k->kont k)))))
+            (make-erl-k
+              :fuel (1- (erl-k->fuel k))
+              :kont (make-kont-fun-call-args
+                      :args (node-fun-call->args
+                              (kont-expr->expr (erl-k->kont k))))))
+           nil)))
   :enable eval-k)
 
 (defrule eval-k-of-expr-fun-call->s
   (implies
-    (and (wf-state-p s)
+    (and (erl-state-p s)
          (erl-k-p k)
-         (> (erl-k->fuel k) 0)
          (equal (kont-kind (erl-k->kont k)) :expr)
          (equal (node-kind (kont-expr->expr (erl-k->kont k))) :fun-call))
     (equal (erl-s-klst->s (eval-k k s))
-           (update-erl-state->in s (make-erl-val-none))))
+           (cond
+            ((not (wf-state-p s)) s)
+            ((not (> (erl-k->fuel k) 0))
+             (update-erl-state->in s (make-erl-val-flimit))) 
+            (t (update-erl-state->in s (make-erl-val-none))))))
   :enable eval-k)
+
 
 ; kont-fun-args
-(defrule eval-k-of-fun-call-args-ok->klst
-  (implies
-    (and (wf-state-p s)
-         (erl-k-p k)
-         (> (erl-k->fuel k) 0)
-         (equal (kont-kind (erl-k->kont k)) :fun-call-args)
-         (erl-fun-p (erl-state->in s)))
-    (equal
-      (erl-s-klst->klst (eval-k k s))
-      (list
-        (make-erl-k
-          :fuel (1- (erl-k->fuel k))
-          :kont (make-kont-expr
-                  :expr (kont-fun-call-args->args (erl-k->kont k))))
-        (make-erl-k
-          :fuel (1- (erl-k->fuel k))
-          :kont (make-kont-fun-call
-                  :fun (erl-state->in s))))))
-  :enable eval-k)
-
-(defrule eval-k-of-fun-call-args-ok->s
-  (implies
-    (and (wf-state-p s) 
-         (erl-k-p k)
-         (> (erl-k->fuel k) 0)
-         (equal (kont-kind (erl-k->kont k)) :fun-call-args)
-         (erl-fun-p (erl-state->in s)))
-    (equal
-      (erl-s-klst->s (eval-k k s))
-      (update-erl-state->in s (make-erl-val-none))))
-  :enable eval-k)
-
-(defrule eval-k-of-fun-call-args-not-fun->klst
-  (implies
-    (and (wf-state-p s) 
-         (erl-k-p k)
-         (> (erl-k->fuel k) 0)
-         (equal (kont-kind (erl-k->kont k)) :fun-call-args)
-         (not (erl-fun-p (erl-state->in s))))
-    (equal (erl-s-klst->klst (eval-k k s)) nil))
-  :enable eval-k)
-
-(defrule eval-k-of-fun-call-args-not-fun->s
-  (implies
-    (and (wf-state-p s)
-         (erl-k-p k)
-         (> (erl-k->fuel k) 0)
-         (equal (kont-kind (erl-k->kont k)) :fun-call-args)
-         (not (erl-fun-p (erl-state->in s))))
-    (equal
-      (erl-s-klst->s (eval-k k s))
-      (update-erl-state->in
-        s
-        (make-erl-val-excpt
-          :err (make-erl-err
-                 :class (make-err-class-error)
-                 :reason (make-exit-reason-badfun
-                           :fun (erl-state->in s)))))))
-  :enable eval-k)
-
-; Combine the results from above to a general rewrite rule.
 (defrule eval-k-of-fun-call-args->klst
   (implies
-    (and (wf-state-p s)
+    (and (erl-state-p s)
          (erl-k-p k)
-         (> (erl-k->fuel k) 0)
          (equal (kont-kind (erl-k->kont k)) :fun-call-args))
     (equal
       (erl-s-klst->klst (eval-k k s))
-      (if (erl-fun-p (erl-state->in s))
+      (if (and (wf-state-p s)
+               (> (erl-k->fuel k) 0)
+               (erl-fun-p (erl-state->in s)))
           (list
             (make-erl-k
               :fuel (1- (erl-k->fuel k))
@@ -121,143 +66,44 @@
               :fuel (1- (erl-k->fuel k))
               :kont (make-kont-fun-call
                       :fun (erl-state->in s))))
-          nil))))
+          nil)))
+  :enable eval-k)
 
-; Combine the results from above to a general rewrite rule.
 (defrule eval-k-of-fun-call-args->s
   (implies
-    (and (wf-state-p s)
+    (and (erl-state-p s)
          (erl-k-p k)
-         (> (erl-k->fuel k) 0)
          (equal (kont-kind (erl-k->kont k)) :fun-call-args))
     (equal
       (erl-s-klst->s (eval-k k s))
-      (if (erl-fun-p (erl-state->in s))
-          (update-erl-state->in s (make-erl-val-none))
-          (update-erl-state->in
-            s
-            (make-erl-val-excpt
-              :err (make-erl-err
+      (cond
+        ((not (wf-state-p s)) s)
+        ((not (> (erl-k->fuel k) 0))
+         (update-erl-state->in s (make-erl-val-flimit)))
+        
+        ((not (erl-fun-p (erl-state->in s)))
+         (update-erl-state->in
+           s
+           (make-erl-val-excpt
+             :err (make-erl-err
                     :class (make-err-class-error)
                     :reason (make-exit-reason-badfun
-                              :fun (erl-state->in s)))))))))
-
-; kont 
-(defrule eval-k-of-fun-call-ok->klst
-  (implies
-    (and (wf-state-p s) 
-         (erl-k-p k)
-         (> (erl-k->fuel k) 0)
-         (equal (kont-kind (erl-k->kont k)) :fun-call)
-         (equal (erl-val-kind (erl-state->in s)) :cons)
-         (mv-nth 1 (eval-fun-call
-                     (update-erl-state->in s (make-erl-val-none))
-                     (kont-fun-call->fun (erl-k->kont k))
-                     (erl-val-cons->lst (erl-state->in s)))))
-    (equal
-      (erl-s-klst->klst (eval-k k s))
-      (list (make-erl-k 
-              :fuel (1- (erl-k->fuel k))
-              :kont (make-kont-exprs :exprs
-                (mv-nth 1 (eval-fun-call
-                    (update-erl-state->in s (make-erl-val-none))
-                    (kont-fun-call->fun (erl-k->kont k))
-                    (erl-val-cons->lst (erl-state->in s))))))
-            (make-erl-k
-              :fuel (1- (erl-k->fuel k)) 
-              :kont (make-kont-function-return 
-                      :bind (erl-state->bind s) 
-                      :module (erl-state->module s))))))
+                              :fun (erl-state->in s))))))
+        (t (update-erl-state->in s (make-erl-val-none))))))
   :enable eval-k)
 
-(defrule eval-k-of-fun-call-ok->s
-  (implies
-    (and (wf-state-p s) 
-         (erl-k-p k)
-         (> (erl-k->fuel k) 0)
-         (equal (kont-kind (erl-k->kont k)) :fun-call)
-         (equal (erl-val-kind (erl-state->in s)) :cons)
-         (mv-nth 1 (eval-fun-call
-                     (update-erl-state->in s (make-erl-val-none))
-                     (kont-fun-call->fun (erl-k->kont k))
-                     (erl-val-cons->lst (erl-state->in s)))))
-    (equal
-      (erl-s-klst->s (eval-k k s))
-      (update-erl-state->in
-        (mv-nth 0 (eval-fun-call
-                    (update-erl-state->in s (make-erl-val-none))
-                    (kont-fun-call->fun (erl-k->kont k))
-                    (erl-val-cons->lst (erl-state->in s))))
-        (make-erl-val-none))))
-  :enable eval-k)
 
-(defrule eval-k-of-fun-call-invalid-args->klst
-  (implies
-    (and (wf-state-p s)
-         (erl-k-p k)
-         (> (erl-k->fuel k) 0)
-         (equal (kont-kind (erl-k->kont k)) :fun-call)
-         (not (equal (erl-val-kind (erl-state->in s)) :cons)))
-    (equal (erl-s-klst->klst (eval-k k s)) nil))
-  :enable eval-k)
-
-(defrule eval-k-of-fun-call-invalid-args->s
-  (implies
-    (and (wf-state-p s)
-         (erl-k-p k)
-         (> (erl-k->fuel k) 0)
-         (equal (kont-kind (erl-k->kont k)) :fun-call)
-         (not (equal (erl-val-kind (erl-state->in s)) :cons)))
-    (equal
-      (erl-s-klst->s (eval-k k s))
-      (update-erl-state->in
-        s
-        (make-erl-val-reject :err "Fun call: invalid arg list."))))
-  :enable eval-k)
-
-(defrule eval-k-of-fun-call-no-clauses->klst
-  (implies
-    (and (wf-state-p s)
-         (erl-k-p k)
-         (> (erl-k->fuel k) 0)
-         (equal (kont-kind (erl-k->kont k)) :fun-call)
-         (equal (erl-val-kind (erl-state->in s)) :cons)
-         (not (mv-nth 1 (eval-fun-call
-                     (update-erl-state->in s (make-erl-val-none))
-                     (kont-fun-call->fun (erl-k->kont k))
-                     (erl-val-cons->lst (erl-state->in s))))))
-    (equal (erl-s-klst->klst (eval-k k s)) nil))
-  :enable eval-k)
-
-(defrule eval-k-of-fun-call-no-clauses->s
-  (implies
-    (and (wf-state-p s)
-         (erl-k-p k)
-         (> (erl-k->fuel k) 0)
-         (equal (kont-kind (erl-k->kont k)) :fun-call)
-         (equal (erl-val-kind (erl-state->in s)) :cons)
-         (not (mv-nth 1 (eval-fun-call
-                     (update-erl-state->in s (make-erl-val-none))
-                     (kont-fun-call->fun (erl-k->kont k))
-                     (erl-val-cons->lst (erl-state->in s))))))
-    (equal
-      (erl-s-klst->s (eval-k k s))
-      (mv-nth 0 (eval-fun-call
-                  (update-erl-state->in s (make-erl-val-none))
-                  (kont-fun-call->fun (erl-k->kont k))
-                  (erl-val-cons->lst (erl-state->in s))))))
-  :enable eval-k)
-
-; Combine the rules from above to a general rewrite rule
+; kont-fun-call 
 (defrule eval-k-of-fun-call->klst
   (implies
-    (and (wf-state-p s)
+    (and (erl-state-p s)
          (erl-k-p k)
-         (> (erl-k->fuel k) 0)
          (equal (kont-kind (erl-k->kont k)) :fun-call))
     (equal
       (erl-s-klst->klst (eval-k k s))
       (cond
+        ((not (wf-state-p s)) nil)
+        ((not (> (erl-k->fuel k) 0)) nil)
         ((not (equal (erl-val-kind (erl-state->in s)) :cons)) nil)
         ((not (mv-nth
                 1 
@@ -269,7 +115,9 @@
         (t (list (make-erl-k 
               :fuel (1- (erl-k->fuel k))
               :kont (make-kont-exprs :exprs
-                (mv-nth 1 (eval-fun-call
+                (mv-nth
+                  1 
+                  (eval-fun-call
                     (update-erl-state->in s (make-erl-val-none))
                     (kont-fun-call->fun (erl-k->kont k))
                     (erl-val-cons->lst (erl-state->in s))))))
@@ -282,13 +130,15 @@
 
 (defrule eval-k-of-fun-call->s
   (implies
-    (and (wf-state-p s)
+    (and (erl-state-p s)
          (erl-k-p k)
-         (> (erl-k->fuel k) 0)
          (equal (kont-kind (erl-k->kont k)) :fun-call))
     (equal
       (erl-s-klst->s (eval-k k s))
       (cond
+        ((not (wf-state-p s)) s)
+        ((not (> (erl-k->fuel k) 0))
+         (update-erl-state->in s (make-erl-val-flimit)))
         ((not (equal (erl-val-kind (erl-state->in s)) :cons)) 
          (update-erl-state->in
            s
@@ -306,8 +156,11 @@
               (kont-fun-call->fun (erl-k->kont k))
               (erl-val-cons->lst (erl-state->in s)))))
         (t (update-erl-state->in
-            (mv-nth 0 (eval-fun-call
-                        (update-erl-state->in s (make-erl-val-none))
-                        (kont-fun-call->fun (erl-k->kont k))
-                        (erl-val-cons->lst (erl-state->in s))))
-            (make-erl-val-none)))))))
+            (mv-nth
+              0 
+              (eval-fun-call
+                (update-erl-state->in s (make-erl-val-none))
+                (kont-fun-call->fun (erl-k->kont k))
+                (erl-val-cons->lst (erl-state->in s))))
+            (make-erl-val-none))))))
+  :enable eval-k)
