acl2/theorems/kont-step/functions.lisp
@@ -3,49 +3,26 @@
 
 ; Function Return Kont-Step ----------------------------------------------------
 
-; Stepping the function-return continuation
-; (defrule eval-k-of-function-return->klst
-;   (implies
-;     (and (wf-state-p s) 
-;          (erl-k-p k)
-;          (> (erl-k->fuel k) 0)
-;          (equal (kont-kind (erl-k->kont k)) :function-return))
-;     (equal (erl-s-klst->klst (eval-k k s)) nil))
-;   :enable eval-k)
-
-; (defrule eval-k-of-function-return->s
-;   (implies
-;     (and (wf-state-p s) 
-;          (erl-k-p k)
-;          (> (erl-k->fuel k) 0)
-;          (equal (kont-kind (erl-k->kont k)) :function-return))
-;     (equal (erl-s-klst->s (eval-k k s))
-;            (update-erl-state->bind-mod
-;             s 
-;             (kont-function-return->bind (erl-k->kont k))
-;             (kont-function-return->module (erl-k->kont k)))))
-;   :enable eval-k)
-
-
-(defrule eval-k-of-function-return->klst-no-constraints
+(defrule eval-k-of-function-return->klst
   (implies
     (and (erl-k-p k)
          (equal (kont-kind (erl-k->kont k)) :function-return))
     (equal (erl-s-klst->klst (eval-k k s)) nil))
   :enable eval-k)
 
-(defrule eval-k-of-function-return->s-no-constraints
+(defrule eval-k-of-function-return->s
   (implies
     (and (erl-state-p s) 
          (erl-k-p k)
          (equal (kont-kind (erl-k->kont k)) :function-return))
-    (equal (erl-s-klst->s (eval-k k s))
-          (cond 
-            ((not (wf-state-p s)) s)
-            ((not (> (erl-k->fuel k) 0)) 
-             (update-erl-state->in s (make-erl-val-flimit)))
-            (t (update-erl-state->bind-mod
-              s 
-              (kont-function-return->bind (erl-k->kont k))
-              (kont-function-return->module (erl-k->kont k)))))))
+    (equal
+      (erl-s-klst->s (eval-k k s))
+      (cond 
+        ((not (wf-state-p s)) s)
+        ((not (> (erl-k->fuel k) 0)) 
+          (update-erl-state->in s (make-erl-val-flimit)))
+        (t (update-erl-state->bind-mod
+          s 
+          (kont-function-return->bind (erl-k->kont k))
+          (kont-function-return->module (erl-k->kont k)))))))
   :enable eval-k)
