acl2/theorems/kont-step/if.lisp
@@ -7,248 +7,101 @@
 ; expression is equivalent to calling the clause-evaluator with no argument for 
 ; pattern matching cases and then continuing with the body of the selected clause.
 
-(defrule eval-k-of-expr-if-ok->klst
-  (implies
-    (and
-       (wf-state-p s) 
-       (erl-k-p k)
-       (> (erl-k->fuel k) 0)
-       (equal (kont-kind (erl-k->kont k)) :expr)
-       (equal (node-kind (kont-expr->expr (erl-k->kont k))) :if)
-       (not (equal (erl-val-kind (erl-state->in
-                      (mv-nth 
-                        0
-                        (eval-clauses 
-                          nil 
-                          (node-if->clauses (kont-expr->expr (erl-k->kont k)))
-                          s))))
-                    :reject))
-       (mv-nth 1 (eval-clauses 
-                  nil 
-                  (node-if->clauses (kont-expr->expr (erl-k->kont k))) s)))
-    (equal 
-      (erl-s-klst->klst (eval-k k s))
-      (list 
-        (make-erl-k 
-          :fuel (1- (erl-k->fuel k))
-          :kont (make-kont-expr 
-            :expr (car (mv-nth 
-                          1
-                          (eval-clauses 
-                            nil
-                            (node-if->clauses (kont-expr->expr (erl-k->kont k))) s)))))
-        (make-erl-k 
-          :fuel (1- (erl-k->fuel k))
-          :kont (make-kont-exprs
-            :exprs (cdr (mv-nth 
-                          1
-                          (eval-clauses
-                            nil
-                            (node-if->clauses (kont-expr->expr (erl-k->kont k))) s))))))))
-  :enable eval-k)
-
-(defrule eval-k-of-expr-if-ok->s
-  (implies
-    (and
-       (wf-state-p s) 
-       (erl-k-p k)
-       (> (erl-k->fuel k) 0)
-       (equal (kont-kind (erl-k->kont k)) :expr)
-       (equal (node-kind (kont-expr->expr (erl-k->kont k))) :if)
-       (not (equal (erl-val-kind (erl-state->in
-                      (mv-nth 
-                        0
-                        (eval-clauses 
-                          nil 
-                          (node-if->clauses (kont-expr->expr (erl-k->kont k)))
-                          s))))
-                    :reject))
-       (mv-nth 1 (eval-clauses 
-                  nil 
-                  (node-if->clauses (kont-expr->expr (erl-k->kont k))) s)))
-    (equal 
-      (erl-s-klst->s (eval-k k s))
-      (update-erl-state->in s (make-erl-val-none))))
-  :enable eval-k)
-
-(defrule eval-k-of-expr-if-reject->klst
-  (implies
-    (and
-       (wf-state-p s) 
-       (erl-k-p k)
-       (> (erl-k->fuel k) 0)
-       (equal (kont-kind (erl-k->kont k)) :expr)
-       (equal (node-kind (kont-expr->expr (erl-k->kont k))) :if)
-       (equal (erl-val-kind (erl-state->in
-                (mv-nth 
-                  0
-                  (eval-clauses 
-                    nil 
-                    (node-if->clauses (kont-expr->expr (erl-k->kont k)))
-                    s))))
-              :reject))
-    (equal (erl-s-klst->klst (eval-k k s)) nil))
-  :enable eval-k)
-
-(defrule eval-k-of-expr-if-reject->s
-  (implies
-    (and
-       (wf-state-p s) 
-       (erl-k-p k)
-       (> (erl-k->fuel k) 0)
-       (equal (kont-kind (erl-k->kont k)) :expr)
-       (equal (node-kind (kont-expr->expr (erl-k->kont k))) :if)
-       (equal (erl-val-kind (erl-state->in
-                (mv-nth 
-                  0
-                  (eval-clauses 
-                    nil 
-                    (node-if->clauses (kont-expr->expr (erl-k->kont k)))
-                    s))))
-              :reject))
-    (equal
-      (erl-s-klst->s (eval-k k s))
-      (mv-nth 
-        0
-        (eval-clauses 
-          nil 
-          (node-if->clauses (kont-expr->expr (erl-k->kont k)))
-          s))))
-  :enable eval-k)
-
-(defrule eval-k-of-expr-if-no-clauses->klst
-  (implies
-    (and
-       (wf-state-p s) 
-       (erl-k-p k)
-       (> (erl-k->fuel k) 0)
-       (equal (kont-kind (erl-k->kont k)) :expr)
-       (equal (node-kind (kont-expr->expr (erl-k->kont k))) :if)
-       (not (equal (erl-val-kind (erl-state->in
-                    (mv-nth 
-                      0
-                      (eval-clauses 
-                        nil 
-                        (node-if->clauses (kont-expr->expr (erl-k->kont k)))
-                        s))))
-              :reject))
-       (not (mv-nth 1 (eval-clauses 
-              nil 
-              (node-if->clauses (kont-expr->expr (erl-k->kont k))) s))))
-    (equal (erl-s-klst->klst (eval-k k s)) nil))
-  :enable eval-k)
-
-(defrule eval-k-of-expr-if-no-clauses->s
-  (implies
-    (and
-       (wf-state-p s) 
-       (erl-k-p k)
-       (> (erl-k->fuel k) 0)
-       (equal (kont-kind (erl-k->kont k)) :expr)
-       (equal (node-kind (kont-expr->expr (erl-k->kont k))) :if)
-       (not (equal (erl-val-kind (erl-state->in
-                    (mv-nth 
-                      0
-                      (eval-clauses 
-                        nil 
-                        (node-if->clauses (kont-expr->expr (erl-k->kont k)))
-                        s))))
-              :reject))
-       (not (mv-nth 1 (eval-clauses 
-              nil 
-              (node-if->clauses (kont-expr->expr (erl-k->kont k))) s))))
-    (equal (erl-s-klst->s (eval-k k s))
-           (update-erl-state->in
-             s
-             (make-erl-val-excpt 
-              :err (make-erl-err :class (make-err-class-error)
-                                 :reason (make-exit-reason-if-clause))))))
-  :enable eval-k)
-
-
-; combine the rules above into a general rewrite rule
 (defrule eval-k-of-expr-if->klst
   (implies
     (and
-       (wf-state-p s) 
+       (erl-state-p s)
        (erl-k-p k)
-       (> (erl-k->fuel k) 0)
        (equal (kont-kind (erl-k->kont k)) :expr)
        (equal (node-kind (kont-expr->expr (erl-k->kont k))) :if))
     (equal
       (erl-s-klst->klst (eval-k k s))
       (cond
-        ((equal (erl-val-kind (erl-state->in
-                  (mv-nth 
-                    0
-                    (eval-clauses 
-                      nil 
-                      (node-if->clauses (kont-expr->expr (erl-k->kont k)))
-                      s))))
-                :reject)
-          nil)
-       ((not (mv-nth 
-              1 
-              (eval-clauses 
-                nil 
+        ((not (wf-state-p s)) nil)
+        ((not (> (erl-k->fuel k) 0)) nil)
+        ((equal
+          (erl-val-kind
+            (erl-state->in
+              (mv-nth 
+                0
+                (eval-clauses 
+                  nil 
+                  (node-if->clauses (kont-expr->expr (erl-k->kont k)))
+                  s))))
+          :reject)
+         nil)
+       ((not (mv-nth
+              1
+              (eval-clauses
+                nil
                 (node-if->clauses (kont-expr->expr (erl-k->kont k))) s)))
         nil)
-      (t 
-       (list 
-        (make-erl-k 
-          :fuel (1- (erl-k->fuel k))
-          :kont (make-kont-expr 
-            :expr (car (mv-nth 
-                          1
-                          (eval-clauses 
-                            nil
-                            (node-if->clauses (kont-expr->expr (erl-k->kont k))) s)))))
-        (make-erl-k 
-          :fuel (1- (erl-k->fuel k))
-          :kont (make-kont-exprs
-            :exprs (cdr (mv-nth 
-                          1
-                          (eval-clauses
-                            nil
-                            (node-if->clauses (kont-expr->expr (erl-k->kont k))) s)))))))
-    
-    )))
+      (t
+       (list
+         (make-erl-k 
+           :fuel (1- (erl-k->fuel k))
+           :kont
+             (make-kont-expr 
+               :expr
+                 (car
+                   (mv-nth
+                     1
+                     (eval-clauses 
+                       nil
+                       (node-if->clauses
+                         (kont-expr->expr (erl-k->kont k))) s)))))
+         (make-erl-k 
+           :fuel (1- (erl-k->fuel k))
+           :kont
+             (make-kont-exprs
+              :exprs
+                (cdr
+                  (mv-nth 
+                    1
+                    (eval-clauses
+                      nil
+                      (node-if->clauses 
+                        (kont-expr->expr (erl-k->kont k))) s))))))))))
     :enable eval-k)
 
 (defrule eval-k-of-expr-if->s
   (implies
     (and
-       (wf-state-p s) 
+       (erl-state-p s) 
        (erl-k-p k)
-       (> (erl-k->fuel k) 0)
        (equal (kont-kind (erl-k->kont k)) :expr)
        (equal (node-kind (kont-expr->expr (erl-k->kont k))) :if))
     (equal
       (erl-s-klst->s (eval-k k s))
       (cond
-        ((equal (erl-val-kind (erl-state->in
-                  (mv-nth 
-                    0
-                    (eval-clauses 
-                      nil 
-                      (node-if->clauses (kont-expr->expr (erl-k->kont k)))
-                      s))))
-                :reject)
-          (mv-nth 
-            0
-            (eval-clauses 
-              nil 
-              (node-if->clauses (kont-expr->expr (erl-k->kont k)))
-              s)))
-       ((not (mv-nth 
-              1 
-              (eval-clauses 
-                nil 
-                (node-if->clauses (kont-expr->expr (erl-k->kont k))) s)))
-        (update-erl-state->in
-          s
-          (make-erl-val-excpt 
-          :err (make-erl-err :class (make-err-class-error)
-                              :reason (make-exit-reason-if-clause)))))
-      (t (update-erl-state->in s (make-erl-val-none))))))
-    :enable eval-k)
+        ((not (wf-state-p s)) s)
+        ((not (> (erl-k->fuel k) 0))
+         (update-erl-state->in s (make-erl-val-flimit)))
+        ((equal
+          (erl-val-kind
+            (erl-state->in
+              (mv-nth 
+                0
+                (eval-clauses 
+                  nil 
+                  (node-if->clauses (kont-expr->expr (erl-k->kont k)))
+                  s))))
+          :reject)
+         (mv-nth 
+           0
+           (eval-clauses 
+             nil 
+             (node-if->clauses (kont-expr->expr (erl-k->kont k)))
+             s)))
+        ((not (mv-nth 
+                1 
+                (eval-clauses 
+                  nil 
+                  (node-if->clauses (kont-expr->expr (erl-k->kont k))) s)))
+         (update-erl-state->in
+           s
+           (make-erl-val-excpt 
+             :err (make-erl-err :class (make-err-class-error)
+                                :reason (make-exit-reason-if-clause)))))
+        (t (update-erl-state->in s (make-erl-val-none))))))
+  :enable eval-k)
