acl2/theorems/kont-step/match.lisp
@@ -10,104 +10,52 @@
 ; expr-match
 (defrule eval-k-of-expr-match->klst
   (implies
-    (and (wf-state-p s)
+    (and (erl-state-p s)
          (erl-k-p k)
-         (> (erl-k->fuel k) 0)
          (equal (kont-kind (erl-k->kont k)) :expr)
          (equal (node-kind (kont-expr->expr (erl-k->kont k))) :match))
     (equal
       (erl-s-klst->klst (eval-k k s))
-      (list
-        (make-erl-k
-          :fuel (1- (erl-k->fuel k))
-          :kont (make-kont-expr
-                  :expr (node-match->rhs
-                           (kont-expr->expr (erl-k->kont k)))))
-        (make-erl-k
-          :fuel (1- (erl-k->fuel k))
-          :kont (make-kont-match
-                  :lhs (node-match->lhs
-                         (kont-expr->expr (erl-k->kont k))))))))
+      (if (and (wf-state-p s) (> (erl-k->fuel k) 0))
+          (list
+            (make-erl-k
+              :fuel (1- (erl-k->fuel k))
+              :kont (make-kont-expr
+                      :expr (node-match->rhs
+                              (kont-expr->expr (erl-k->kont k)))))
+            (make-erl-k
+              :fuel (1- (erl-k->fuel k))
+              :kont (make-kont-match
+                      :lhs (node-match->lhs
+                            (kont-expr->expr (erl-k->kont k))))))
+          nil)))
   :enable eval-k)
 
 (defrule eval-k-of-expr-match->s
   (implies
-    (and (wf-state-p s)
+    (and (erl-state-p s)
          (erl-k-p k)
-         (> (erl-k->fuel k) 0)
          (equal (kont-kind (erl-k->kont k)) :expr)
          (equal (node-kind (kont-expr->expr (erl-k->kont k))) :match))
     (equal (erl-s-klst->s (eval-k k s))
-           (update-erl-state->in s (make-erl-val-none))))
+           (cond
+             ((not (wf-state-p s)) s)
+             ((not (> (erl-k->fuel k) 0))
+              (update-erl-state->in s (make-erl-val-flimit)))
+             (t (update-erl-state->in s (make-erl-val-none))))))
   :enable eval-k)
+
 
 ; kont-match
 (defrule eval-k-of-match->klst
   (implies 
-    (and
-       (wf-state-p s) 
-       (erl-k-p k)
-       (> (erl-k->fuel k) 0)
-       (equal (kont-kind (erl-k->kont k)) :match))
+    (and (erl-state-p s) 
+         (erl-k-p k)
+         (equal (kont-kind (erl-k->kont k)) :match))
     (equal (erl-s-klst->klst (eval-k k s)) nil))
   :enable eval-k)
 
-(defrule eval-k-of-match-ok->s
-  (implies 
-    (and
-       (wf-state-p s) 
-       (erl-k-p k)
-       (> (erl-k->fuel k) 0)
-       (equal (kont-kind (erl-k->kont k)) :match)
-       (not (and (equal (erl-val-kind (erl-state->in (eval-match (kont-match->lhs (erl-k->kont k)) s))) :excpt)
-                 (equal (exit-reason-kind 
-                          (erl-err->reason (erl-val-excpt->err (erl-state->in (eval-match (kont-match->lhs (erl-k->kont k)) s))))) 
-                        :badmatch))))
-    (equal (erl-s-klst->s (eval-k k s)) (eval-match (kont-match->lhs (erl-k->kont k)) s)))
-  :enable eval-k)
-
-(defrule eval-k-of-match-badmatch->s
-  (implies 
-    (and
-       (wf-state-p s) 
-       (erl-k-p k)
-       (> (erl-k->fuel k) 0)
-       (equal (kont-kind (erl-k->kont k)) :match)
-       (and (equal (erl-val-kind (erl-state->in (eval-match (kont-match->lhs (erl-k->kont k)) s))) :excpt)
-            (equal (exit-reason-kind 
-                    (erl-err->reason (erl-val-excpt->err (erl-state->in (eval-match (kont-match->lhs (erl-k->kont k)) s))))) 
-                  :badmatch)))
-    (equal (erl-s-klst->s (eval-k k s))
-           (update-erl-state->in
-             s
-             (make-erl-val-excpt 
-               :err (make-erl-err :class (make-err-class-error) 
-                                  :reason (make-exit-reason-badmatch :val (erl-state->in s)))))))
-  :enable eval-k)
-
-; Combined to general rewrite rule
 (defrule eval-k-of-match->s
-  (implies 
-    (and
-       (wf-state-p s) 
-       (erl-k-p k)
-       (> (erl-k->fuel k) 0)
-       (equal (kont-kind (erl-k->kont k)) :match))
-    (equal 
-      (erl-s-klst->s (eval-k k s)) 
-      (if (not (and (equal (erl-val-kind (erl-state->in (eval-match (kont-match->lhs (erl-k->kont k)) s))) :excpt)
-                    (equal (exit-reason-kind 
-                              (erl-err->reason (erl-val-excpt->err (erl-state->in (eval-match (kont-match->lhs (erl-k->kont k)) s))))) 
-                            :badmatch)))
-          (eval-match (kont-match->lhs (erl-k->kont k)) s)
-          (update-erl-state->in
-             s
-             (make-erl-val-excpt 
-               :err (make-erl-err :class (make-err-class-error) 
-                                  :reason (make-exit-reason-badmatch :val (erl-state->in s))))))))
-  :enable eval-k)
-
-(defrule eval-k-of-match->s-no-constraint
   (implies 
     (and
        (erl-state-p s) 
@@ -117,15 +65,27 @@
       (erl-s-klst->s (eval-k k s)) 
       (cond 
         ((not (wf-state-p s)) s)
-        ((not (> (erl-k->fuel k) 0)) (update-erl-state->in s (make-erl-val-flimit)))
-        ((not (and (equal (erl-val-kind (erl-state->in (eval-match (kont-match->lhs (erl-k->kont k)) s))) :excpt)
-                    (equal (exit-reason-kind 
-                              (erl-err->reason (erl-val-excpt->err (erl-state->in (eval-match (kont-match->lhs (erl-k->kont k)) s))))) 
-                            :badmatch)))
+        ((not (> (erl-k->fuel k) 0))
+         (update-erl-state->in s (make-erl-val-flimit)))
+        ((not 
+          (and 
+            (equal
+              (erl-val-kind 
+                (erl-state->in 
+                  (eval-match (kont-match->lhs (erl-k->kont k)) s)))
+              :excpt)
+            (equal
+              (exit-reason-kind 
+                (erl-err->reason
+                  (erl-val-excpt->err
+                    (erl-state->in
+                      (eval-match (kont-match->lhs (erl-k->kont k)) s))))) 
+              :badmatch)))
           (eval-match (kont-match->lhs (erl-k->kont k)) s))
         (t (update-erl-state->in
              s
              (make-erl-val-excpt 
                :err (make-erl-err :class (make-err-class-error) 
-                                  :reason (make-exit-reason-badmatch :val (erl-state->in s)))))))))
+                                  :reason (make-exit-reason-badmatch
+                                            :val (erl-state->in s)))))))))
   :enable eval-k)
