acl2/theorems/kont-step/remote-call.lisp
@@ -7,211 +7,117 @@
 ; expression is equivalent to evaluating the arguments in order, and then invoking
 ; the call evaluator which will then provide the body of the function to execute.
 
+; expr-remote-call
 (defrule eval-k-of-expr-remote-call->klst
   (implies
-    (and (wf-state-p s) 
+    (and (erl-state-p s) 
          (erl-k-p k)
-         (> (erl-k->fuel k) 0)
          (equal (kont-kind (erl-k->kont k)) :expr)
          (equal (node-kind (kont-expr->expr (erl-k->kont k))) :remote-call))
     (equal 
       (erl-s-klst->klst (eval-k k s))
-      (list
-        (make-erl-k
-          :fuel (1- (erl-k->fuel k))
-          :kont (make-kont-expr 
-            :expr (node-remote-call->args (kont-expr->expr (erl-k->kont k)))))
-        (make-erl-k
-          :fuel (1- (erl-k->fuel k))
-          :kont (make-kont-remote-call
-                  :module (node-remote-call->module (kont-expr->expr (erl-k->kont k)))
-                  :call (node-remote-call->fn (kont-expr->expr (erl-k->kont k))))))))
+      (if (and (wf-state-p s) (> (erl-k->fuel k) 0))
+          (list
+            (make-erl-k
+              :fuel (1- (erl-k->fuel k))
+              :kont (make-kont-expr
+                      :expr (node-remote-call->args
+                              (kont-expr->expr (erl-k->kont k)))))
+            (make-erl-k
+              :fuel (1- (erl-k->fuel k))
+              :kont (make-kont-remote-call
+                      :module (node-remote-call->module
+                                (kont-expr->expr (erl-k->kont k)))
+                      :call (node-remote-call->fn
+                              (kont-expr->expr (erl-k->kont k))))))
+          nil)))
   :enable eval-k)
 
 (defrule eval-k-of-expr-remote-call->s
   (implies
-    (and (wf-state-p s) 
+    (and (erl-state-p s) 
          (erl-k-p k)
-         (> (erl-k->fuel k) 0)
          (equal (kont-kind (erl-k->kont k)) :expr)
          (equal (node-kind (kont-expr->expr (erl-k->kont k))) :remote-call))
     (equal 
       (erl-s-klst->s (eval-k k s))
-      (update-erl-state->in s (make-erl-val-none))))
-  :enable eval-k)
-
-(defrule eval-k-of-remote-call-ok->klst
-  (implies
-    (and (wf-state-p s) 
-         (erl-k-p k)
-         (> (erl-k->fuel k) 0)
-         (equal (kont-kind (erl-k->kont k)) :remote-call)
-         (equal (erl-val-kind (erl-state->in s)) :cons)
-         (mv-nth 1 (eval-remote-call
-                     (update-erl-state->in s (make-erl-val-none))
-                     (kont-remote-call->module (erl-k->kont k))
-                     (kont-remote-call->call (erl-k->kont k))
-                     (erl-val-cons->lst (erl-state->in s)))))
-    (equal
-      (erl-s-klst->klst (eval-k k s))
-      (list (make-erl-k 
-              :fuel (1- (erl-k->fuel k))
-              :kont (make-kont-exprs :exprs
-                (mv-nth 1 (eval-remote-call
-                    (update-erl-state->in s (make-erl-val-none))
-                    (kont-remote-call->module (erl-k->kont k))
-                    (kont-remote-call->call (erl-k->kont k))
-                    (erl-val-cons->lst (erl-state->in s))))))
-            (make-erl-k
-              :fuel (1- (erl-k->fuel k)) 
-              :kont (make-kont-function-return 
-                      :bind (erl-state->bind s) 
-                      :module (erl-state->module s))))))
-  :enable eval-k)
-
-(defrule eval-k-of-remote-call-ok->s
-  (implies
-    (and (wf-state-p s) 
-         (erl-k-p k)
-         (> (erl-k->fuel k) 0)
-         (equal (kont-kind (erl-k->kont k)) :remote-call)
-         (equal (erl-val-kind (erl-state->in s)) :cons)
-         (mv-nth 1 (eval-remote-call
-                     (update-erl-state->in s (make-erl-val-none))
-                     (kont-remote-call->module (erl-k->kont k))
-                     (kont-remote-call->call (erl-k->kont k))
-                     (erl-val-cons->lst (erl-state->in s)))))
-    (equal
-      (erl-s-klst->s (eval-k k s))
-      (update-erl-state->in 
-        (mv-nth 0 (eval-remote-call
-                    (update-erl-state->in s (make-erl-val-none))
-                    (kont-remote-call->module (erl-k->kont k))
-                    (kont-remote-call->call (erl-k->kont k))
-                    (erl-val-cons->lst (erl-state->in s))))
-        (make-erl-val-none))))
-  :enable eval-k)
-
-(defrule eval-k-of-remote-call-invalid-args->klst
-  (implies
-    (and (wf-state-p s) 
-         (erl-k-p k)
-         (> (erl-k->fuel k) 0)
-         (equal (kont-kind (erl-k->kont k)) :remote-call)
-         (not (equal (erl-val-kind (erl-state->in s)) :cons)))
-    (equal (erl-s-klst->klst (eval-k k s)) nil))
-  :enable eval-k)
-
-(defrule eval-k-of-remote-call-invalid-args->s
-  (implies
-    (and (wf-state-p s) 
-         (erl-k-p k)
-         (> (erl-k->fuel k) 0)
-         (equal (kont-kind (erl-k->kont k)) :remote-call)
-         (not (equal (erl-val-kind (erl-state->in s)) :cons)))
-    (equal 
-      (erl-s-klst->s (eval-k k s))
-      (update-erl-state->in 
-        s
-        (make-erl-val-reject :err "Remote call: invalid arg list."))))
-  :enable eval-k)
-
-(defrule eval-k-of-remote-call-no-clauses->klst
-  (implies
-    (and (wf-state-p s) 
-         (erl-k-p k)
-         (> (erl-k->fuel k) 0)
-         (equal (kont-kind (erl-k->kont k)) :remote-call)
-         (equal (erl-val-kind (erl-state->in s)) :cons)
-         (not (mv-nth 1 (eval-remote-call
-                     (update-erl-state->in s (make-erl-val-none))
-                     (kont-remote-call->module (erl-k->kont k))
-                     (kont-remote-call->call (erl-k->kont k))
-                     (erl-val-cons->lst (erl-state->in s))))))
-    (equal (erl-s-klst->klst (eval-k k s)) nil))
-  :enable eval-k)
-
-(defrule eval-k-of-remote-call-no-clauses->s
-  (implies
-    (and (wf-state-p s) 
-         (erl-k-p k)
-         (> (erl-k->fuel k) 0)
-         (equal (kont-kind (erl-k->kont k)) :remote-call)
-         (equal (erl-val-kind (erl-state->in s)) :cons)
-         (not (mv-nth 1 (eval-remote-call
-                     (update-erl-state->in s (make-erl-val-none))
-                     (kont-remote-call->module (erl-k->kont k))
-                     (kont-remote-call->call (erl-k->kont k))
-                     (erl-val-cons->lst (erl-state->in s))))))
-    (equal 
-      (erl-s-klst->s (eval-k k s))
-      (mv-nth 0 (eval-remote-call
-                     (update-erl-state->in s (make-erl-val-none))
-                     (kont-remote-call->module (erl-k->kont k))
-                     (kont-remote-call->call (erl-k->kont k))
-                     (erl-val-cons->lst (erl-state->in s))))))
+      (cond
+        ((not (wf-state-p s)) s)
+        ((not (> (erl-k->fuel k) 0))
+         (update-erl-state->in s (make-erl-val-flimit)))
+        (t (update-erl-state->in s (make-erl-val-none))))))
   :enable eval-k)
 
 
-; Combine the rules from above to a general rewrite rule
+; kont-remote-call
 (defrule eval-k-of-remote->klst
   (implies
-    (and (wf-state-p s) 
+    (and (erl-state-p s) 
          (erl-k-p k)
-         (> (erl-k->fuel k) 0)
          (equal (kont-kind (erl-k->kont k)) :remote-call))
     (equal
       (erl-s-klst->klst (eval-k k s))
-      (cond ((not (equal (erl-val-kind (erl-state->in s)) :cons)) nil)
-            ((not (mv-nth 1 (eval-remote-call
-                              (update-erl-state->in s (make-erl-val-none))
-                              (kont-remote-call->module (erl-k->kont k))
-                              (kont-remote-call->call (erl-k->kont k))
-                              (erl-val-cons->lst (erl-state->in s)))))
-              nil)
-            (t (list (make-erl-k 
-                      :fuel (1- (erl-k->fuel k))
-                      :kont (make-kont-exprs :exprs
-                        (mv-nth 1 (eval-remote-call
+      (cond
+        ((not (wf-state-p s)) nil)
+        ((not (> (erl-k->fuel k) 0)) nil)
+        ((not (equal (erl-val-kind (erl-state->in s)) :cons)) nil)
+        ((not (mv-nth 1 (eval-remote-call
+                          (update-erl-state->in s (make-erl-val-none))
+                          (kont-remote-call->module (erl-k->kont k))
+                          (kont-remote-call->call (erl-k->kont k))
+                          (erl-val-cons->lst (erl-state->in s)))))
+          nil)
+        (t (list
+             (make-erl-k 
+               :fuel (1- (erl-k->fuel k))
+               :kont (make-kont-exprs
+                       :exprs
+                         (mv-nth
+                          1 
+                          (eval-remote-call
                             (update-erl-state->in s (make-erl-val-none))
                             (kont-remote-call->module (erl-k->kont k))
                             (kont-remote-call->call (erl-k->kont k))
                             (erl-val-cons->lst (erl-state->in s))))))
-                    (make-erl-k
-                      :fuel (1- (erl-k->fuel k)) 
-                      :kont (make-kont-function-return 
-                              :bind (erl-state->bind s) 
-                              :module (erl-state->module s))))))))
+             (make-erl-k
+               :fuel (1- (erl-k->fuel k)) 
+               :kont (make-kont-function-return 
+                       :bind (erl-state->bind s) 
+                       :module (erl-state->module s))))))))
   :enable eval-k)
 
 (defrule eval-k-of-remote->s
   (implies
-    (and (wf-state-p s) 
+    (and (erl-state-p s) 
          (erl-k-p k)
-         (> (erl-k->fuel k) 0)
          (equal (kont-kind (erl-k->kont k)) :remote-call))
     (equal
       (erl-s-klst->s (eval-k k s))
-      (cond ((not (equal (erl-val-kind (erl-state->in s)) :cons))
-             (update-erl-state->in 
-              s
-              (make-erl-val-reject :err "Remote call: invalid arg list.")))
-            ((not (mv-nth 1 (eval-remote-call
-                              (update-erl-state->in s (make-erl-val-none))
-                              (kont-remote-call->module (erl-k->kont k))
-                              (kont-remote-call->call (erl-k->kont k))
-                              (erl-val-cons->lst (erl-state->in s)))))
-             (mv-nth 
-              0 
-              (eval-remote-call
-                (update-erl-state->in s (make-erl-val-none))
-                (kont-remote-call->module (erl-k->kont k))
-                (kont-remote-call->call (erl-k->kont k))
-                (erl-val-cons->lst (erl-state->in s)))))
-            (t (update-erl-state->in 
-                 (mv-nth 0 (eval-remote-call
-                             (update-erl-state->in s (make-erl-val-none))
-                             (kont-remote-call->module (erl-k->kont k))
-                             (kont-remote-call->call (erl-k->kont k))
-                             (erl-val-cons->lst (erl-state->in s))))
-                 (make-erl-val-none)))))))
+      (cond 
+        ((not (wf-state-p s)) s)
+        ((not (> (erl-k->fuel k) 0))
+         (update-erl-state->in s (make-erl-val-flimit)))
+        ((not (equal (erl-val-kind (erl-state->in s)) :cons))
+         (update-erl-state->in 
+           s
+           (make-erl-val-reject :err "Remote call: invalid arg list.")))
+        ((not (mv-nth 1 (eval-remote-call
+                          (update-erl-state->in s (make-erl-val-none))
+                          (kont-remote-call->module (erl-k->kont k))
+                          (kont-remote-call->call (erl-k->kont k))
+                          (erl-val-cons->lst (erl-state->in s)))))
+         (mv-nth 
+           0 
+           (eval-remote-call
+             (update-erl-state->in s (make-erl-val-none))
+             (kont-remote-call->module (erl-k->kont k))
+             (kont-remote-call->call (erl-k->kont k))
+             (erl-val-cons->lst (erl-state->in s)))))
+        (t (update-erl-state->in 
+             (mv-nth 0 (eval-remote-call
+                         (update-erl-state->in s (make-erl-val-none))
+                         (kont-remote-call->module (erl-k->kont k))
+                         (kont-remote-call->call (erl-k->kont k))
+                         (erl-val-cons->lst (erl-state->in s))))
+             (make-erl-val-none))))))
+  :enable eval-k)
