acl2/theorems/kont-step/tuple.lisp
@@ -3,140 +3,92 @@
 
 ; Tuple Kont-Step --------------------------------------------------------------
 
-
 ; The following theorems show that evaluating a continuation for a tuple
 ; expression is equivalent to evaluating every element of the tuple from
 ; left to right, and then merging the results.
 
-(defrule eval-k-of-expr-tuple-empty->klst
+(defrule eval-k-of-expr-tuple->s
   (implies
-    (and (wf-state-p s)
+    (and (erl-state-p s)
          (erl-k-p k)
-         (> (erl-k->fuel k) 0)
          (equal (kont-kind (erl-k->kont k)) :expr)
-         (equal (node-kind (kont-expr->expr (erl-k->kont k))) :tuple)
-         (null (node-tuple->lst (kont-expr->expr (erl-k->kont k)))))
-    (equal (erl-s-klst->klst (eval-k k s)) nil))
-  :enable eval-k)
-
-(defrule eval-k-of-expr-tuple-empty->s
-  (implies
-    (and (wf-state-p s)
-         (erl-k-p k)
-         (> (erl-k->fuel k) 0)
-         (equal (kont-kind (erl-k->kont k)) :expr)
-         (equal (node-kind (kont-expr->expr (erl-k->kont k))) :tuple)
-         (null (node-tuple->lst (kont-expr->expr (erl-k->kont k)))))
-    (equal (erl-s-klst->s (eval-k k s))
-           (update-erl-state->in
-             s
-             (make-erl-val-tuple :lst nil))))
+         (equal (node-kind (kont-expr->expr (erl-k->kont k))) :tuple))
+    (equal
+      (erl-s-klst->s (eval-k k s))
+      
+      (cond
+        ((not (wf-state-p s)) s)
+        ((not (> (erl-k->fuel k) 0))
+         (update-erl-state->in s (make-erl-val-flimit)))
+        ((not (consp (node-tuple->lst (kont-expr->expr (erl-k->kont k)))))
+         (update-erl-state->in s (make-erl-val-tuple :lst nil)))
+        (t (update-erl-state->in s (make-erl-val-none))))))
   :enable eval-k)
 
 (defrule eval-k-of-expr-tuple->klst
   (implies
-    (and (wf-state-p s)
+    (and (erl-state-p s)
          (erl-k-p k)
-         (> (erl-k->fuel k) 0)
          (equal (kont-kind (erl-k->kont k)) :expr)
-         (equal (node-kind (kont-expr->expr (erl-k->kont k))) :tuple)
-         (consp (node-tuple->lst (kont-expr->expr (erl-k->kont k)))))
+         (equal (node-kind (kont-expr->expr (erl-k->kont k))) :tuple))
     (equal
       (erl-s-klst->klst (eval-k k s))
-      (list
-        (make-erl-k
-          :fuel (1- (erl-k->fuel k))
-          :kont (make-kont-expr
-                  :expr (car (node-tuple->lst
-                               (kont-expr->expr (erl-k->kont k))))))
-        (make-erl-k
-          :fuel (1- (erl-k->fuel k))
-          :kont (make-kont-tuple
-                  :t-rem (make-node-tuple
-                           :lst (cdr (node-tuple->lst
-                                       (kont-expr->expr (erl-k->kont k)))))
-                  :bind-0 (erl-state->bind s))))))
+      (if (and (wf-state-p s)
+               (> (erl-k->fuel k) 0)
+               (node-tuple->lst (kont-expr->expr (erl-k->kont k))))
+          (list
+            (make-erl-k
+              :fuel (1- (erl-k->fuel k))
+              :kont (make-kont-expr
+                      :expr (car (node-tuple->lst
+                                   (kont-expr->expr (erl-k->kont k))))))
+            (make-erl-k
+              :fuel (1- (erl-k->fuel k))
+              :kont (make-kont-tuple
+                      :t-rem (make-node-tuple
+                              :lst (cdr (node-tuple->lst
+                                          (kont-expr->expr (erl-k->kont k)))))
+                      :bind-0 (erl-state->bind s))))
+          nil)))
   :enable eval-k)
-
-(defrule eval-k-of-expr-tuple->s
-  (implies
-    (and (wf-state-p s)
-         (erl-k-p k)
-         (> (erl-k->fuel k) 0)
-         (equal (kont-kind (erl-k->kont k)) :expr)
-         (equal (node-kind (kont-expr->expr (erl-k->kont k))) :tuple)
-         (consp (node-tuple->lst (kont-expr->expr (erl-k->kont k)))))
-    (equal (erl-s-klst->s (eval-k k s))
-           (update-erl-state->in s (make-erl-val-none))))
-  :enable eval-k)
-
-; merge the rules from above to a general rewrite rule
-(defrule eval-k-of-expr-tuple-ok->klst
-  (implies
-    (and (wf-state-p s)
-         (erl-k-p k)
-         (> (erl-k->fuel k) 0)
-         (equal (kont-kind (erl-k->kont k)) :expr)
-         (equal (node-kind (kont-expr->expr (erl-k->kont k))) :tuple))
-    (equal (erl-s-klst->klst (eval-k k s))
-           (if (node-tuple->lst (kont-expr->expr (erl-k->kont k)))
-               (list
-                (make-erl-k
-                  :fuel (1- (erl-k->fuel k))
-                  :kont (make-kont-expr
-                          :expr (car (node-tuple->lst
-                                      (kont-expr->expr (erl-k->kont k))))))
-                (make-erl-k
-                  :fuel (1- (erl-k->fuel k))
-                  :kont (make-kont-tuple
-                          :t-rem (make-node-tuple
-                                  :lst (cdr (node-tuple->lst
-                                              (kont-expr->expr (erl-k->kont k)))))
-                          :bind-0 (erl-state->bind s))))
-              nil))))
-
-(defrule eval-k-of-expr-tuple-ok->s
-  (implies
-    (and (wf-state-p s)
-         (erl-k-p k)
-         (> (erl-k->fuel k) 0)
-         (equal (kont-kind (erl-k->kont k)) :expr)
-         (equal (node-kind (kont-expr->expr (erl-k->kont k))) :tuple))
-    (equal (erl-s-klst->s (eval-k k s))
-           (if (node-tuple->lst (kont-expr->expr (erl-k->kont k)))
-               (update-erl-state->in s (make-erl-val-none))
-               (update-erl-state->in s (make-erl-val-tuple :lst nil))))))
 
 
 ; kont-tuple
 (defrule eval-k-of-tuple->klst
   (implies 
-    (and (wf-state-p s) 
+    (and (erl-state-p s) 
          (erl-k-p k)
-         (> (erl-k->fuel k) 0)
          (equal (kont-kind (erl-k->kont k)) :tuple))
-    (equal (erl-s-klst->klst (eval-k k s))
-           (list (make-erl-k 
-                    :fuel (1- (erl-k->fuel k)) 
-                    :kont (make-kont-expr :expr (kont-tuple->t-rem (erl-k->kont k))))
-                 (make-erl-k 
-                    :fuel (1- (erl-k->fuel k))
-                    :kont (make-kont-tuple-merge 
-                            :t-hd (erl-state->in s)
-                            :t-bind (erl-state->bind s))))))
+    (equal
+      (erl-s-klst->klst (eval-k k s))
+      (if (and (wf-state-p s) (> (erl-k->fuel k) 0)) 
+          (list (make-erl-k 
+                  :fuel (1- (erl-k->fuel k)) 
+                  :kont (make-kont-expr 
+                        :expr (kont-tuple->t-rem (erl-k->kont k))))
+                (make-erl-k 
+                  :fuel (1- (erl-k->fuel k))
+                  :kont (make-kont-tuple-merge 
+                          :t-hd (erl-state->in s)
+                          :t-bind (erl-state->bind s))))
+          nil)))
   :enable eval-k)
 
 (defrule eval-k-of-tuple->s
   (implies 
-    (and (wf-state-p s) 
+    (and (erl-state-p s) 
          (erl-k-p k)
-         (> (erl-k->fuel k) 0)
          (equal (kont-kind (erl-k->kont k)) :tuple))
     (equal (erl-s-klst->s (eval-k k s))
-           (update-erl-state->bind 
-             s
-             (kont-tuple->bind-0 (erl-k->kont k)))))
+           (cond
+             ((not (wf-state-p s) ) s)
+             ((not (> (erl-k->fuel k) 0))
+              (update-erl-state->in s (make-erl-val-flimit)))
+             (t (update-erl-state->bind 
+                  s
+                  (kont-tuple->bind-0 (erl-k->kont k)))))))
   :enable eval-k)
+
 
 ; kont-tuple-merge
 (defrule eval-k-of-tuple-merge->klst
@@ -144,60 +96,6 @@
     (and (erl-k-p k)
          (equal (kont-kind (erl-k->kont k)) :tuple-merge))
     (equal (erl-s-klst->klst (eval-k k s)) nil))
-  :enable eval-k)
-
-(defrule eval-k-of-tuple-merge-ok->s
-  (implies
-    (and (wf-state-p s)
-         (erl-k-p k)
-         (> (erl-k->fuel k) 0)
-         (equal (kont-kind (erl-k->kont k)) :tuple-merge)
-         (equal (erl-val-kind (erl-state->in s)) :tuple)
-         (omap::compatiblep (erl-state->bind s)
-                            (kont-tuple-merge->t-bind (erl-k->kont k))))
-    (equal
-      (erl-s-klst->s (eval-k k s))
-      (update-erl-state->in-bind
-        s
-        (make-erl-val-tuple
-          :lst (cons (kont-tuple-merge->t-hd (erl-k->kont k))
-                     (erl-val-tuple->lst (erl-state->in s))))
-        (omap::update*
-          (erl-state->bind s)
-          (kont-tuple-merge->t-bind (erl-k->kont k))))))
-  :enable eval-k)
-
-(defrule eval-k-of-tuple-merge-bad-tuple->s
-  (implies
-    (and (wf-state-p s)
-         (erl-k-p k)
-         (> (erl-k->fuel k) 0)
-         (equal (kont-kind (erl-k->kont k)) :tuple-merge)
-         (not (equal (erl-val-kind (erl-state->in s)) :tuple)))
-    (equal
-      (erl-s-klst->s (eval-k k s))
-      (update-erl-state->in 
-        s 
-        (make-erl-val-reject :err "tuple-merge expects tuple"))))
-  :enable eval-k)
-
-(defrule eval-k-of-tuple-merge-incomaptible->s
-  (implies
-    (and (wf-state-p s)
-         (erl-k-p k)
-         (> (erl-k->fuel k) 0)
-         (equal (kont-kind (erl-k->kont k)) :tuple-merge)
-         (equal (erl-val-kind (erl-state->in s)) :tuple)
-         (not (omap::compatiblep (erl-state->bind s)
-                            (kont-tuple-merge->t-bind (erl-k->kont k)))))
-    (equal
-      (erl-s-klst->s (eval-k k s))
-      (update-erl-state->in 
-        s 
-        (make-erl-val-excpt 
-          :err (make-erl-err :class (make-err-class-error) 
-                             :reason (make-exit-reason-badmatch 
-                                        :val (erl-state->in s)))))))
   :enable eval-k)
 
 (defrule eval-k-of-tuple-merge->s
@@ -209,7 +107,8 @@
       (erl-s-klst->s (eval-k k s))
       (cond
         ((not (wf-state-p s)) s)
-        ((zp (erl-k->fuel k)) (update-erl-state->in s (make-erl-val-flimit)))
+        ((not (> (erl-k->fuel k) 0))
+         (update-erl-state->in s (make-erl-val-flimit)))
         ((not (equal (erl-val-kind (erl-state->in s)) :tuple))
          (update-erl-state->in 
             s 
@@ -218,11 +117,11 @@
                 (erl-state->bind s)
                 (kont-tuple-merge->t-bind (erl-k->kont k))))
          (update-erl-state->in 
-          s 
-          (make-erl-val-excpt 
-            :err (make-erl-err :class (make-err-class-error) 
-                               :reason (make-exit-reason-badmatch 
-                                        :val (erl-state->in s))))))
+           s 
+           (make-erl-val-excpt 
+             :err (make-erl-err :class (make-err-class-error) 
+                                :reason (make-exit-reason-badmatch 
+                                          :val (erl-state->in s))))))
         (t (update-erl-state->in-bind
              s
              (make-erl-val-tuple
@@ -230,4 +129,5 @@
                           (erl-val-tuple->lst (erl-state->in s))))
              (omap::update*
                (erl-state->bind s)
-               (kont-tuple-merge->t-bind (erl-k->kont k)))))))))
+               (kont-tuple-merge->t-bind (erl-k->kont k))))))))
+  :enable eval-k)
