acl2/theorems/kont-step/unop.lisp
@@ -1,7 +1,6 @@
 (in-package "ACL2")
 (include-book "../core/eval-theorems")
 
-
 ; Unop Kont-Step ---------------------------------------------------------------
 
 ; The following theorems show that evaluating a continuation for a unop 
@@ -9,26 +8,28 @@
 ; the unop, as would happen in Erlang's control flow.
 ; There are also some rules about excpetions, rejections, etc. 
 
+; expr-unop
 (defrule eval-k-of-expr-unop->klst
   (implies
-    (and (wf-state-p s)
+    (and (erl-state-p s)
          (erl-k-p k)
-         (> (erl-k->fuel k) 0)
          (equal (kont-kind (erl-k->kont k)) :expr)
          (equal (node-kind (kont-expr->expr (erl-k->kont k))) :unop))
     (equal
       (erl-s-klst->klst (eval-k k s))
-      (list
-        (make-erl-k
-          :fuel (1- (erl-k->fuel k))
-          :kont (make-kont-expr
-                  :expr (node-unop->expr
-                           (kont-expr->expr (erl-k->kont k)))))
-        (make-erl-k
-          :fuel (1- (erl-k->fuel k))
-          :kont (make-kont-unop
-                  :op (node-unop->op
-                        (kont-expr->expr (erl-k->kont k))))))))
+      (if (and (wf-state-p s) (> (erl-k->fuel k) 0))
+          (list
+            (make-erl-k
+              :fuel (1- (erl-k->fuel k))
+              :kont (make-kont-expr
+                      :expr (node-unop->expr
+                              (kont-expr->expr (erl-k->kont k)))))
+            (make-erl-k
+              :fuel (1- (erl-k->fuel k))
+              :kont (make-kont-unop
+                      :op (node-unop->op
+                            (kont-expr->expr (erl-k->kont k))))))
+          nil)))
   :enable eval-k)
 
 (defrule eval-k-of-expr-unop->s
@@ -39,14 +40,19 @@
          (equal (kont-kind (erl-k->kont k)) :expr)
          (equal (node-kind (kont-expr->expr (erl-k->kont k))) :unop))
     (equal (erl-s-klst->s (eval-k k s))
-           (update-erl-state->in s (make-erl-val-none))))
+           (cond
+             ((not (wf-state-p s)) s)
+             ((not (> (erl-k->fuel k) 0))
+              (update-erl-state->in s (make-erl-val-flimit)))
+             (t (update-erl-state->in s (make-erl-val-none))))))
   :enable eval-k)
 
+
+; kont-unop
 (defrule eval-k-of-unop->klst
   (implies
-    (and (wf-state-p s)
+    (and (erl-state-p s)
          (erl-k-p k)
-         (> (erl-k->fuel k) 0)
          (equal (kont-kind (erl-k->kont k)) :unop))
     (equal (erl-s-klst->klst (eval-k k s)) nil))
   :enable eval-k)
@@ -59,9 +65,13 @@
          (equal (kont-kind (erl-k->kont k)) :unop))
     (equal
       (erl-s-klst->s (eval-k k s))
-      (update-erl-state->in
-        s
-        (apply-erl-unop
-          (kont-unop->op (erl-k->kont k))
-          (erl-state->in s)))))
+      (cond
+        ((not (wf-state-p s)) s)
+        ((not (> (erl-k->fuel k) 0))
+        (update-erl-state->in s (make-erl-val-flimit)))
+        (t (update-erl-state->in
+             s
+             (apply-erl-unop
+               (kont-unop->op (erl-k->kont k))
+               (erl-state->in s)))))))
   :enable eval-k)
