acl2/theorems/state/module.lisp
@@ -1,0 +1,37 @@
+(in-package "ACL2")
+(include-book "../core/eval-theorems")
+
+(set-induction-depth-limit 1)
+
+; Erl-State Module Theorems ----------------------------------------------------
+
+; The theorems below reason about what happens the module field of an erl-state
+; after various operations.
+
+(defrule erl-state->module-of-eval-match
+  (implies
+    (erl-state-p s)
+    (equal (erl-state->module (eval-match p s))
+           (erl-state->module s)))
+  :enable eval-match)
+
+(defrule erl-state->module-of-match-args
+  (implies
+    (erl-state-p s)
+    (equal (erl-state->module (match-args cs args s))
+           (erl-state->module s)))
+  :enable match-args)
+
+(defrule erl-state->module-of-eval-clauses-when-consp
+  (implies
+    (erl-state-p s)
+    (equal (erl-state->module (mv-nth 0 (eval-clauses-when-consp args cls s)))
+           (erl-state->module s)))
+  :enable eval-clauses-when-consp)
+
+(defrule erl-state->module-of-eval-clauses
+  (implies
+    (erl-state-p s)
+    (equal (erl-state->module (mv-nth 0 (eval-clauses args cls s)))
+           (erl-state->module s)))
+  :enable eval-clauses)
