acl2/theorems/state/world.lisp
@@ -1,0 +1,75 @@
+(in-package "ACL2")
+(include-book "../core/eval-theorems")
+
+(set-induction-depth-limit 1)
+
+; Erl-State World Theorems -----------------------------------------------------
+
+; The theorems below reason about what happens the world field of an erl-state
+; after various operations.
+
+(defrule erl-state->world-of-eval-match
+  (implies
+    (erl-state-p s)
+    (equal (erl-state->world (eval-match p s))
+           (erl-state->world s)))
+  :enable eval-match)
+
+(defrule erl-state->world-of-match-args
+  (implies
+    (erl-state-p s)
+    (equal (erl-state->world (match-args cs args s))
+           (erl-state->world s)))
+  :enable match-args)
+
+(defrule erl-state->world-of-eval-clauses-when-consp
+  (implies
+    (erl-state-p s)
+    (equal (erl-state->world (mv-nth 0 (eval-clauses-when-consp args cls s)))
+           (erl-state->world s)))
+  :enable eval-clauses-when-consp)
+
+(defrule erl-state->world-of-eval-clauses
+  (implies
+    (erl-state-p s)
+    (equal (erl-state->world (mv-nth 0 (eval-clauses args cls s)))
+           (erl-state->world s)))
+  :enable eval-clauses)
+
+(defrule erl-state->world-of-eval-local-call
+  (implies
+    (erl-state-p s)
+    (equal (erl-state->world (mv-nth 0 (eval-local-call s c args)))
+           (erl-state->world s)))
+  :enable eval-local-call)
+
+(defrule erl-state->world-of-eval-remote-call
+  (implies
+    (erl-state-p s)
+    (equal (erl-state->world (mv-nth 0 (eval-remote-call s m c args)))
+           (erl-state->world s)))
+  :enable eval-remote-call)
+
+(defrule erl-state->world-of-eval-fun-call
+  (implies
+    (erl-state-p s)
+    (equal (erl-state->world (mv-nth 0 (eval-fun-call s f args)))
+           (erl-state->world s)))
+  :enable eval-fun-call)
+
+; The world field of an erl-state never changes during evaluation.
+(defrule apply-k-of-world
+  (implies 
+    (and (erl-klst-p klst) (erl-state-p s))
+    (equal (erl-state->world (apply-k s klst))
+           (erl-state->world s)))
+  :expand (eval-k (car klst) s)
+  :enable (apply-k)
+  :disable (apply-k-of-step apply-k-of-consp))
+
+(defrule eval-k-of-world
+  (implies 
+    (and (erl-k-p k) (erl-state-p s))
+    (equal (erl-state->world (erl-s-klst->s (eval-k k s)))
+           (erl-state->world s)))
+  :enable eval-k)
