acl2/theorems/top.lisp
@@ -2,4 +2,4 @@
 
 (include-book "core/top")
 (include-book "kont-step/top")
-(include-book "state/state")
+(include-book "state/top")
